Checkpoint rewrite to do fix specs and cleanup proofs.
The specs for describing DstFileExists where too lose: the user of the spec
couldn't conclude that the only thing that changed in the directory tree was the
creation of the destination file.

Many dirtree lemmas are unproven, but maybe let it be, because we are switching
to Haogang's dirtrees.

Todo: eliminate a few easy admits and update FS.delete spec (maybe that also
should be done in the disklog2 branch).

src/App.v
@@ -66,6 +66,8 @@ Proof.
   intuition.
 Qed.
 
+
+
 Lemma nodup_app_eq_notin: forall name d (dents : list (string *
   DIRTREE.dirtree)), NoDup (map fst ((name, d) :: dents)) ->  ~ In name (map fst dents).
 Proof.
@@ -177,7 +179,7 @@ Proof.
     destruct (string_dec s temp_fn).
     apply notin_map in H.
     intuition.
-    rewrite IHtree_elem.
+   rewrite IHtree_elem.
     reflexivity.
     apply notin_map in H.
     intuition.
@@ -294,7 +296,7 @@ Proof.
 Qed.
 
   
-Lemma dirtree_find_add_dents: forall temp_fn elem tree_elem,
+Lemma find_dirlist_add_dents: forall temp_fn elem tree_elem,
   DIRTREE.find_dirlist temp_fn (DIRTREE.add_to_list temp_fn elem tree_elem)
   = Some elem.
 Proof.
@@ -370,7 +372,7 @@ Qed.
 
 
 Lemma dirtree_prune_add_dents: forall inum dents temp_fn elem tree_elem,
-  ~ In temp_fn (map fst tree_elem)                                 
+  ~ In temp_fn (map fst tree_elem)
   -> dents = (DIRTREE.add_to_list temp_fn elem tree_elem)
   -> DIRTREE.tree_prune inum dents [] temp_fn
         (DIRTREE.TreeDir inum dents) = DIRTREE.TreeDir inum tree_elem.
@@ -455,80 +457,258 @@ Proof.
 Qed.
 
 
-Lemma find_name_elem_update_exists : forall dnum tree_elem name i b a,
-     In name (map fst tree_elem) ->
-       DIRTREE.find_name [name]
-                         (DIRTREE.TreeDir dnum
-                                          (map
-                                             (DIRTREE.update_subtree_helper
-                                                (fun _ : DIRTREE.dirtree => DIRTREE.TreeFile i b a)
-                                                name) tree_elem)) = Some (i, false).
-Proof.
-Admitted.
+(* maybe don't need these *)
 
-Lemma fold_right_impl_in_elem: forall tree_elem fn elem,
-  In fn (map fst tree_elem) ->
-  fold_right
-     (DIRTREE.find_subtree_helper (fun tree : DIRTREE.dirtree => Some tree)
-                                  fn) None tree_elem = Some elem.
-Proof.
-Admitted.
-  
-
-Lemma find_name_impl_in_elem : forall name dnum tree_elem inum,
-     DIRTREE.find_name [name] (DIRTREE.TreeDir dnum tree_elem) = Some (inum, false) ->
-     In name (map fst tree_elem).
-Proof.
-  (* use above *)
-Admitted.
-
-Lemma find_name_impl_find_subtree: forall name inum tree a b,
-    DIRTREE.find_name [name] tree = Some (inum, false) ->                                   
-      DIRTREE.find_subtree [name] tree = Some (DIRTREE.TreeFile inum b a).
-Proof.
-Admitted.
-
-
-Lemma find_name_update_dents: forall dnum temp_fn tree_elem inum b elem,
-  In temp_fn (map fst tree_elem) ->
-  DIRTREE.find_name [temp_fn]
-     (DIRTREE.TreeDir dnum
-     (map (DIRTREE.update_subtree_helper
-             (fun _ : DIRTREE.dirtree => elem) temp_fn) tree_elem)) = Some (inum, b).
-Proof.
-  (* use find_update_dents *)
-Admitted.
-
-
-Lemma find_subtree_fold_right_update_ne: forall fn1 fn2 dnum tree_elem elem inum bytes attr, 
+Lemma find_subtree_fold_right_add_ne: forall fn1 fn2 tree_elem elem,
   fn1 <> fn2 ->
-  DIRTREE.find_subtree [fn1] (DIRTREE.TreeDir dnum tree_elem) = elem ->
   fold_right
      (DIRTREE.find_subtree_helper (fun tree : DIRTREE.dirtree => Some tree)
         fn1) None
-     (map
-        (DIRTREE.update_subtree_helper
-           (fun _ : DIRTREE.dirtree => DIRTREE.TreeFile inum bytes attr)
-           fn2) tree_elem) = elem.
-Proof.
-Admitted.
-   
-Lemma find_name_add_to_list: forall fn dnum tree_elem inum, 
-   DIRTREE.find_name [fn] (DIRTREE.TreeDir dnum tree_elem) = None ->
-   DIRTREE.find_name [fn]
-     (DIRTREE.TreeDir dnum
-        (DIRTREE.add_to_list fn
-                             (DIRTREE.TreeFile inum [] BYTEFILE.attr0) tree_elem)) =  Some (inum, false).
+     (DIRTREE.add_to_list fn2 elem tree_elem) =
+  fold_right
+     (DIRTREE.find_subtree_helper (fun tree : DIRTREE.dirtree => Some tree)
+        fn1) None tree_elem.
 Proof.
 Admitted.
 
-Lemma find_name_delete_from_list: forall fn dnum tree_elem w, 
-   DIRTREE.find_name [fn] (DIRTREE.TreeDir dnum tree_elem) = Some (w, false) ->
-   DIRTREE.find_name [fn]
-     (DIRTREE.TreeDir dnum
-        (DIRTREE.delete_from_list fn tree_elem)) =  None.
+  
+Lemma find_subtree_fold_right_add: forall fn tree_elem elem,
+  fold_right
+     (DIRTREE.find_subtree_helper (fun tree : DIRTREE.dirtree => Some tree)
+        fn) None
+     (DIRTREE.add_to_list fn elem tree_elem) = Some elem.
 Proof.
 Admitted.
+
+
+(* new ones *)
+
+Lemma find_name_impl_find_subtree: forall name inum tree a b,
+  DIRTREE.find_name [name] tree = Some (inum, false) ->                                   
+    DIRTREE.find_subtree [name] tree = Some (DIRTREE.TreeFile inum b a).
+Proof.
+Admitted.
+
+
+Lemma find_subtree_impl_find_name: forall name inum tree a b,
+  DIRTREE.find_subtree [name] tree = Some (DIRTREE.TreeFile inum b a) ->
+  DIRTREE.find_name [name] tree = Some (inum, false).
+Proof.
+Admitted.
+
+Lemma find_subtree_update_subtree: forall fn tree elem0 elem1,
+  DIRTREE.find_subtree [fn] tree = Some (elem0) ->
+  DIRTREE.find_subtree [fn] (DIRTREE.update_subtree [fn] elem1 tree) = Some (elem1).
+Proof.
+Admitted.
+
+
+Lemma update_update_subtree_eq: forall fn elem0 elem1 tree,
+  DIRTREE.update_subtree [fn] elem1 (DIRTREE.update_subtree [fn] elem0 tree) =
+  DIRTREE.update_subtree [fn] elem1 tree.
+Proof.      
+Admitted.
+
+Lemma find_name_not_present: forall fn tree_elem dnum,
+  ~In fn (map fst tree_elem) ->
+  DIRTREE.find_name [fn] (DIRTREE.TreeDir dnum tree_elem) = None.
+Proof.
+Admitted.
+
+
+Lemma find_root_finds_root: forall dents dnum,
+  DIRTREE.find_subtree [] (DIRTREE.TreeDir dnum dents) = Some (DIRTREE.TreeDir dnum dents).
+Proof.
+  intros.
+  unfold DIRTREE.find_subtree.
+  reflexivity.
+Qed.
+
+Lemma find_root_impl_tree_is_root: forall tree dents dnum,
+  DIRTREE.find_subtree [] tree =
+  Some (DIRTREE.TreeDir dnum dents) ->
+  tree = DIRTREE.TreeDir dnum dents.
+Proof.
+Admitted.
+
+Lemma find_tree_eq_root_impl_tree_is_root: forall tree dents dnum,
+  DIRTREE.find_subtree [] tree = DIRTREE.find_subtree [] (DIRTREE.TreeDir dnum dents) ->
+  tree = (DIRTREE.TreeDir dnum dents).
+Proof.
+  intros.
+  unfold DIRTREE.find_subtree in H.
+  inversion H.
+  reflexivity.
+Qed.
+
+
+(* Some lemmas about root directory.  A few can be generalized to take pathnames instead of 
+ being specialized to root. *)
+
+Parameter the_dnum : addr.
+
+Definition rep_root tree dents :=
+  tree = DIRTREE.TreeDir the_dnum dents.
+
+Lemma root_has_rep_root: forall dents,
+  rep_root (DIRTREE.TreeDir the_dnum dents) dents.
+Proof.
+  intros.
+  unfold rep_root.
+  reflexivity.
+Qed.  
+
+Lemma find_name_add_root_dents_ne: forall fn1 fn2 dents telem,
+  fn1 <> fn2 ->
+  DIRTREE.find_name [fn1] (DIRTREE.TreeDir the_dnum 
+                                             (DIRTREE.add_to_list fn2 telem dents)) =
+  DIRTREE.find_name [fn1]  (DIRTREE.TreeDir the_dnum dents).
+Proof.
+  intros.
+Admitted.
+
+Lemma find_root_add_to_list: forall dents fn telem,
+  DIRTREE.find_subtree [] (DIRTREE.TreeDir the_dnum (DIRTREE.add_to_list fn telem dents)) =
+  Some (DIRTREE.TreeDir the_dnum (DIRTREE.add_to_list fn telem dents)).
+Proof.
+Admitted.
+
+Lemma find_subtree_add_root_dents: forall fn dents telem,
+  DIRTREE.find_subtree [fn] (DIRTREE.TreeDir the_dnum 
+                                             (DIRTREE.add_to_list fn telem dents)) =
+  Some telem.
+Proof.
+  intros.
+Admitted.
+
+Lemma find_root_graft_dents: forall fn dnum dents elem,
+  DIRTREE.find_subtree []
+        (DIRTREE.tree_graft dnum dents [] fn elem (DIRTREE.TreeDir dnum dents)) =
+  Some (DIRTREE.TreeDir dnum (DIRTREE.add_to_list fn elem dents)).
+Proof.
+Admitted.
+
+
+Lemma delete_from_dir_add_dents: forall fn telem dents,
+   DIRTREE.delete_from_dir fn
+     (DIRTREE.TreeDir the_dnum
+                      (DIRTREE.add_to_list fn telem dents)) =
+   DIRTREE.TreeDir the_dnum dents.
+Proof.
+  intros.
+Admitted.
+
+
+Lemma delete_graft_root_dents: forall fn dents telem,
+   DIRTREE.delete_from_dir fn
+    (DIRTREE.tree_graft the_dnum dents [] fn telem (DIRTREE.TreeDir the_dnum dents)) =
+   DIRTREE.TreeDir the_dnum dents.
+Proof.
+  intros.
+Admitted.
+
+Lemma find_name_delete_from_dir: forall fn tree dents telem, 
+  DIRTREE.find_name [fn] (DIRTREE.TreeDir the_dnum dents) = None ->
+  DIRTREE.find_name [fn]
+         (DIRTREE.delete_from_dir fn
+            (DIRTREE.tree_graft the_dnum dents [] fn telem tree)) = None.
+
+Proof.
+Admitted.
+
+
+Lemma find_root_prune_add_list: forall fn telem dents,
+  DIRTREE.find_subtree []
+       (DIRTREE.tree_prune the_dnum (DIRTREE.add_to_list fn telem dents) [] fn
+                            (DIRTREE.TreeDir the_dnum (DIRTREE.add_to_list fn telem  dents))) =
+  Some (DIRTREE.TreeDir the_dnum dents).
+Proof.
+  intros.
+Admitted.
+
+
+Lemma update_subtree_graft_dents: forall fn dnum dents elem1 elem0,
+  DIRTREE.find_name [fn] (DIRTREE.TreeDir dnum dents) = None ->
+  DIRTREE.update_subtree [fn] elem1
+   (DIRTREE.tree_graft dnum dents [] fn elem0 (DIRTREE.TreeDir dnum dents)) =
+  DIRTREE.tree_graft dnum dents [] fn elem1 (DIRTREE.TreeDir dnum dents).
+Proof.
+Admitted.
+
+Lemma find_subtree_graft_dents: forall fn dnum dents elem,
+  DIRTREE.find_subtree [fn]
+      (DIRTREE.tree_graft dnum dents [] fn elem (DIRTREE.TreeDir dnum dents)) =
+  Some elem.
+Proof.
+Admitted.
+
+
+Lemma find_name_graft_dents: forall fn dnum dents tinum b a,
+  DIRTREE.find_name [fn]
+                    (DIRTREE.tree_graft dnum dents [] fn (DIRTREE.TreeFile tinum b a)
+                                        (DIRTREE.TreeDir dnum dents)) =
+  Some (tinum, false).
+Proof.
+Admitted.
+
+Lemma find_subtree_graft_dents_ne: forall fn1 fn2 dnum dents elem,
+  fn1 <> fn2 ->
+  DIRTREE.find_subtree [fn1]
+     (DIRTREE.tree_graft dnum dents [] fn2 elem (DIRTREE.TreeDir dnum dents)) =
+  DIRTREE.find_subtree [fn1] (DIRTREE.TreeDir dnum dents).
+Proof.
+Admitted.
+
+Lemma find_name_graft_dents_ne: forall fn1 fn2 dnum dents elem,
+  fn1 <> fn2 ->
+  DIRTREE.find_name [fn1]
+     (DIRTREE.tree_graft dnum dents [] fn2 elem (DIRTREE.TreeDir dnum dents)) =
+  DIRTREE.find_name [fn1] (DIRTREE.TreeDir dnum dents).
+Proof.
+Admitted.
+
+
+Lemma prune_add_root_dents: forall fn dents telem,
+  DIRTREE.tree_prune the_dnum
+    (DIRTREE.add_to_list fn telem dents) []  fn (DIRTREE.TreeDir the_dnum
+                                           (DIRTREE.add_to_list fn telem dents)) =
+  DIRTREE.TreeDir the_dnum dents.
+Proof.
+Admitted.
+
+Lemma graft_root_is_add_root_dents: forall fn dents telem,
+  DIRTREE.tree_graft the_dnum dents [] fn telem
+                     (DIRTREE.TreeDir the_dnum dents) =
+  DIRTREE.TreeDir the_dnum (DIRTREE.add_to_list fn telem dents).
+Proof.
+Admitted.
+
+Lemma  update_subtree_root: forall root_new root_old,
+  DIRTREE.update_subtree [] root_new root_old = root_new.
+Proof.
+  intros.
+  unfold DIRTREE.update_subtree; eauto.
+Qed.
+
+Opaque DIRTREE.tree_graft.
+Opaque DIRTREE.update_subtree.
+Opaque DIRTREE.find_subtree.
+Opaque DIRTREE.find_name.
+Opaque DIRTREE.add_to_dir.
+Opaque DIRTREE.delete_from_dir.
+
+(* XXX in Log? *)
+Lemma would_recover_either_pimpl_pred : forall xp F old (newpred: pred),
+  newpred (list2mem old) ->
+  LOG.would_recover_either xp F old old =p=> LOG.would_recover_either_pred xp F old newpred.
+Proof.
+  intros.
+  unfold LOG.would_recover_either, LOG.would_recover_either_pred.
+  cancel.
+  rewrite <- LOG.would_recover_either'_pred'_pimpl.
+  instantiate(d0:= old).
+  cancel.
+Qed.
 
 
 (**
@@ -566,133 +746,10 @@ Proof.
   apply  wordToNat_natToWord_idempotent' in H1.
   rewrite H1; auto.
   auto.
-  admit.
+  eauto.
+  (* exact Rec.Rec.data BYTEFILE.byte_type. *)
 Admitted.
 
-    
-
-Parameter the_dnum : addr.
-Definition temp_fn := ".temp"%string.
-
-(* The file system may crash during a transaction while running atomic_cp or
-atomic_cp_recover. The state of the file system after a crash can be described
-by the following 3 generic states and 6 type of transactions between those 3
-states: *)
-
-Inductive state :=
-| NoTempFile
-| TempFileExists
-| DstFileExists
-.
-
-Inductive transition :=
-| NoTemp2NoTemp
-| NoTemp2Temp
-| Temp2Temp
-| Temp2NoTemp
-| Temp2Dst
-| Dst2Dst
-.
-
-Definition rep_root tree tree_elem :=
-  DIRTREE.find_subtree [] tree = Some (DIRTREE.TreeDir the_dnum tree_elem).
-  
-Definition rep_tree st (tree: DIRTREE.dirtree) src_fn dst_fn temp_fn :=
-  match st with
-    | NoTempFile =>
-      exists tree_elem, rep_root tree tree_elem /\
-                             DIRTREE.find_name [temp_fn] tree = None
-    | TempFileExists =>
-      exists tinum old_inum bytes attr tree_elem,
-         rep_root tree tree_elem /\
-         DIRTREE.find_subtree [src_fn] tree = Some (DIRTREE.TreeFile old_inum bytes attr) /\
-         DIRTREE.find_name [temp_fn] tree = Some (tinum, false)
-    | DstFileExists =>
-      exists old_tree old_inum new_inum bytes attr tree_elem,
-        rep_root tree tree_elem /\  rep_root old_tree tree_elem /\
-          DIRTREE.find_subtree [src_fn] old_tree = Some (DIRTREE.TreeFile old_inum bytes attr) /\
-          tree = DIRTREE.tree_graft the_dnum tree_elem [] dst_fn (DIRTREE.TreeFile new_inum bytes attr) old_tree  /\
-          DIRTREE.find_name [temp_fn] tree = None
-  end.
-
-
-Definition rep_crash (t : transition) Fm Ftop fsxp src_fn dst_fn :=
-  (match t with
-     | NoTemp2NoTemp =>
-       exists m' tree',
-         [[ (Fm * DIRTREE.rep fsxp Ftop tree')%pred (list2mem m') ]] *
-         [[rep_tree NoTempFile tree' src_fn dst_fn temp_fn]] *
-         LOG.would_recover_either_pred (FSXPLog fsxp) (sb_rep fsxp) m'
-             (exists tree'',
-                       (Fm * DIRTREE.rep fsxp Ftop tree'') * 
-                       [[rep_tree NoTempFile tree'' src_fn dst_fn temp_fn]])
-     | NoTemp2Temp =>
-       exists m' tree',
-         [[ (Fm * DIRTREE.rep fsxp Ftop tree')%pred (list2mem m') ]] *
-         [[rep_tree NoTempFile tree' src_fn dst_fn temp_fn]] *
-         LOG.would_recover_either_pred (FSXPLog fsxp) (sb_rep fsxp) m'
-             (exists tree'',
-                       (Fm * DIRTREE.rep fsxp Ftop tree'') * 
-                       [[rep_tree TempFileExists tree'' src_fn dst_fn temp_fn ]])
-     | Temp2NoTemp =>
-       exists m' tree',
-         [[ (Fm * DIRTREE.rep fsxp Ftop tree')%pred (list2mem m') ]] *
-         [[rep_tree TempFileExists tree' src_fn dst_fn temp_fn ]] *
-         LOG.would_recover_either_pred (FSXPLog fsxp) (sb_rep fsxp) m'
-             (exists tree'',
-                       (Fm * DIRTREE.rep fsxp Ftop tree'') * 
-                       [[rep_tree NoTempFile tree'' src_fn dst_fn temp_fn ]])
-     | Temp2Temp =>
-       exists m' tree',
-        [[ (Fm * DIRTREE.rep fsxp Ftop tree')%pred (list2mem m') ]] *
-        [[rep_tree TempFileExists tree' src_fn dst_fn temp_fn ]] *
-        LOG.would_recover_either_pred (FSXPLog fsxp) (sb_rep fsxp) m'
-           (exists tree'',
-              (Fm * DIRTREE.rep fsxp Ftop tree'') *
-              [[rep_tree TempFileExists tree'' src_fn dst_fn temp_fn ]])
-     | Temp2Dst =>
-       exists m' tree',
-        [[ (Fm * DIRTREE.rep fsxp Ftop tree')%pred (list2mem m') ]] *
-        [[rep_tree TempFileExists tree' src_fn dst_fn temp_fn ]] *
-        LOG.would_recover_either_pred (FSXPLog fsxp) (sb_rep fsxp) m'
-            (exists tree'',
-                        (Fm * DIRTREE.rep fsxp Ftop tree'') * 
-                        [[rep_tree DstFileExists tree'' src_fn dst_fn temp_fn ]])
-     | Dst2Dst =>
-       exists m' tree',
-        [[ (Fm * DIRTREE.rep fsxp Ftop tree')%pred (list2mem m') ]] *
-        [[rep_tree DstFileExists tree' src_fn dst_fn temp_fn ]] *
-        LOG.would_recover_either_pred (FSXPLog fsxp) (sb_rep fsxp) m'
-            (exists tree'',
-                        (Fm * DIRTREE.rep fsxp Ftop tree'') * 
-                        [[rep_tree DstFileExists tree'' src_fn dst_fn temp_fn ]])
-
-   end)%pred.
-
-Definition tree_reps tree src_fn dst_fn   :=
-  rep_tree NoTempFile tree src_fn dst_fn temp_fn  \/
-  rep_tree TempFileExists tree src_fn dst_fn temp_fn  \/
-  rep_tree DstFileExists tree src_fn dst_fn temp_fn .
-
-Definition crash_transitions Fm Ftop fsxp src_fn dst_fn  :=
-  (rep_crash NoTemp2NoTemp Fm Ftop fsxp src_fn dst_fn  \/
-   rep_crash NoTemp2Temp Fm Ftop fsxp src_fn dst_fn  \/
-   rep_crash Temp2NoTemp Fm Ftop fsxp src_fn dst_fn  \/
-   rep_crash Temp2Temp Fm Ftop fsxp src_fn dst_fn  \/
-   rep_crash Temp2Dst Fm Ftop fsxp src_fn dst_fn \/
-   rep_crash Dst2Dst Fm Ftop fsxp src_fn dst_fn )%pred.
-
-Lemma would_recover_either_pimpl_pred : forall xp F old (newpred: pred),
-  newpred (list2mem old) ->
-  LOG.would_recover_either xp F old old =p=> LOG.would_recover_either_pred xp F old newpred.
-Proof.
-  intros.
-  unfold LOG.would_recover_either, LOG.would_recover_either_pred.
-  cancel.
-  rewrite <- LOG.would_recover_either'_pred'_pimpl.
-  instantiate(d0:= old).
-  cancel.
-Qed.
 
 (* copy an existing src into an existing, empty dst. *)
 Definition copy2temp T fsxp src_inum dst_inum mscs rx : prog T :=
@@ -704,204 +761,824 @@ Definition copy2temp T fsxp src_inum dst_inum mscs rx : prog T :=
   let^ (mscs, ok1) <- FS.file_set_attr fsxp dst_inum sattr mscs;   (* then set_attr *)
   rx ^(mscs, ok && ok1).
 
-Ltac crash_prolog := match goal with
-    | [ |- _ * LOG.would_recover_either_pred  _ _ _ _ =p=> _ ] => idtac "recover"; unfold rep_crash, rep_tree; subst; pimpl_crash; norm
-end.
-
-Ltac crash_epilog := match goal with
-      | [ |- stars _ * stars _ =p=> stars _ ] => idtac "unfold"; simpl; cancel; eapply LOG.would_recover_either_pred_ppimpl; eapply pimpl_exists_l; intro; cancel; eexists
-    end.
-
-Ltac would_recover_either2pred :=
-  match goal with
-    | [ |- LOG.would_recover_either _ _ ?m  _  =p=> LOG.would_recover_either_pred _ _ ?m _ ] => idtac "either2pred";
-          eapply would_recover_either_pimpl_pred; eexists; instantiate (x := (DIRTREE.TreeDir the_dnum _)); eapply sep_star_lift_apply'; eauto
-  end.
-
-
-Ltac src_fn_exists :=
-  match goal with
-    | [ H:  fold_right (DIRTREE.find_subtree_helper (fun tree : DIRTREE.dirtree => Some tree) ?src_fn)
-       None ?tree_elem = Some (DIRTREE.TreeFile _ _ _) |- 
-       fold_right (DIRTREE.find_subtree_helper (fun tree : DIRTREE.dirtree => Some tree) ?src_fn) None
-           ?tree_elem = Some (DIRTREE.TreeFile _ _ _)] => rewrite H; eauto
-  end.
-
-Ltac src_fn_exists_tree :=
-  match goal with 
-  | [ |- DIRTREE.find_subtree [?src_fn] (DIRTREE.TreeDir _ ?tree_elem) = Some (DIRTREE.TreeFile _ _ _)] =>
-      unfold DIRTREE.find_subtree; simpl; auto; src_fn_exists
-  end.
-
-
-Ltac temp_fn_exists :=
-  match goal with 
-  | [ H :  DIRTREE.find_name [temp_fn] (DIRTREE.TreeDir _ ?tree_elem) = Some (_, _)
-    |- DIRTREE.find_name [temp_fn] (DIRTREE.TreeDir _ ?tree_elem) = Some (_, _)] => rewrite H; eauto
-  end.
-
-Ltac crush_would_recover_either tree_elem := would_recover_either2pred;
-      try repeat (eexists); try src_fn_exists; try temp_fn_exists.
-  
-Ltac crush_exists_crash := try repeat (eexists);try src_fn_exists; try temp_fn_exists.
-
-Theorem copy2temp_ok : forall fsxp src_fn dst_fn src_inum temp_inum mscs,
-  {< m Fm Ftop tree tree_elem attr bytes,
+Theorem copy2temp_ok : forall fsxp src_inum tinum mscs,
+  {< m Fm Ftop temp_tree src_fn tfn bytes attr,
   PRE  LOG.rep (FSXPLog fsxp) (sb_rep fsxp) (NoTransaction m) mscs * 
-        [[ (Fm * DIRTREE.rep fsxp Ftop tree)%pred (list2mem m) ]] *
-        [[ tree = DIRTREE.TreeDir the_dnum tree_elem ]] *
-        [[ src_fn <> temp_fn ]] *
-        [[ DIRTREE.find_subtree [src_fn] tree = Some (DIRTREE.TreeFile src_inum bytes attr) ]] *
-        [[ DIRTREE.find_name [temp_fn] tree = Some (temp_inum, false) ]]
+        [[ (Fm * DIRTREE.rep fsxp Ftop temp_tree)%pred (list2mem m) ]] *
+        [[ DIRTREE.find_subtree [src_fn] temp_tree =
+           Some (DIRTREE.TreeFile src_inum bytes attr) ]] *
+        [[ DIRTREE.find_subtree [tfn] temp_tree =
+           Some (DIRTREE.TreeFile tinum [] BYTEFILE.attr0) ]]
   POST RET:^(mscs, r)
     exists m' tree',
       LOG.rep (FSXPLog fsxp) (sb_rep fsxp) (NoTransaction m') mscs *
       [[ (Fm * DIRTREE.rep fsxp Ftop tree')%pred (list2mem m') ]] *
-      (([[r = false ]] * 
-          [[ DIRTREE.find_name [temp_fn] tree' =  Some (temp_inum, false) ]]) \/
+      (([[r = false ]] * ([[tree' = temp_tree]] \/
+        (exists b a,  
+        [[ tree' = DIRTREE.update_subtree [tfn] (DIRTREE.TreeFile tinum b a) temp_tree ]]))) \/
        ([[r = true ]] *
-        [[ tree' = DIRTREE.update_subtree [temp_fn]
-                                          (DIRTREE.TreeFile temp_inum bytes attr) tree ]]))
+        [[ tree' = DIRTREE.update_subtree [tfn] (DIRTREE.TreeFile tinum bytes attr) temp_tree ]]))
    CRASH
-     rep_crash Temp2Temp Fm Ftop fsxp src_fn dst_fn
-  >} copy2temp fsxp src_inum temp_inum mscs.
+     (LOG.would_recover_either (FSXPLog fsxp) (sb_rep fsxp) m m) \/
+     LOG.would_recover_either_pred (FSXPLog fsxp) (sb_rep fsxp) m (
+       exists tree' b a,
+         (Fm * DIRTREE.rep fsxp Ftop tree') *
+         [[ tree' = DIRTREE.update_subtree [tfn] (DIRTREE.TreeFile tinum b a) temp_tree ]])  \/
+    (exists m' tree' b a,
+       [[ (Fm * DIRTREE.rep fsxp Ftop tree')%pred (list2mem m') ]] *
+       [[ tree' = DIRTREE.update_subtree [tfn] (DIRTREE.TreeFile tinum b a) temp_tree ]] *
+       LOG.would_recover_either_pred (FSXPLog fsxp) (sb_rep fsxp) m' (exists tree'' b' a',
+         (Fm * DIRTREE.rep fsxp Ftop tree'') *
+         [[ tree'' = DIRTREE.update_subtree [tfn] (DIRTREE.TreeFile tinum b' a') temp_tree ]]))
+  >} copy2temp fsxp src_inum tinum mscs.
 Proof.
   unfold copy2temp; intros.
-  step. (* file_get_sz *)
-  instantiate (pathname := [src_fn]).
-  eauto.
-  step.  (* get_attr *)
-  instantiate (pathname := [src_fn]).
-  eauto.
-  step. (* read_bytes *)
-  instantiate (pathname := [src_fn]).
-  eauto.
-
+  (* file_get_sz *)
+  step.
+  (* get_attr *)  
+  step.
+  (* read_bytes *)
+  step.
   (* append step instantiates incorrectly *)
   eapply pimpl_ok2. eauto with prog. cancel.
-  instantiate (pathname := [temp_fn]).
-  instantiate (bytes0 := []).
-  instantiate (attr0 := BYTEFILE.attr0).
-  eauto.
-  eapply find_name_impl_find_subtree; eauto.
+  instantiate (pathname := [tfn]); eauto.
   instantiate (Fi := emp).
   constructor.
   eauto.
 
   (* sattr and its preconditions. *)
   eapply pimpl_ok2. eauto with prog. cancel.
-  instantiate (pathname := [temp_fn]).
-  instantiate (bytes0 := []).
-  instantiate (attr0 := BYTEFILE.attr0).
-  eapply find_name_impl_find_subtree; eauto.
+  instantiate (pathname := [tfn]); eauto.
 
-  destruct a9.
   (* two return cases after setattr failed *)
+  destruct a9.
   step.
+  step.
+  cancel.
+  right.
+  pred_apply.
   eapply pimpl_or_r; left.
+  eapply LOG.would_recover_either_pred_ppimpl.
+  eapply pimpl_exists_l; intro.
+  repeat (apply pimpl_exists_r; eexists).
   cancel.
-  rewrite find_name_update_dents with (inum := temp_inum) (b := false); eauto.
-  eapply find_name_impl_in_elem; eauto.
+  rewrite <- H7; auto.
+  instantiate (pathname0 := [tfn]).
+  eapply find_subtree_update_subtree;eauto.
+
   step.
-
-  crash_prolog.
-  instantiate (m' := m).
-  crash_epilog.
-  instantiate (tinum := temp_inum).
-  rewrite H7.
-  rewrite find_name_elem_update_exists; auto.
-  repeat (eexists).
-
-  erewrite find_subtree_fold_right_update_ne.
-  instantiate (old_inum := src_inum); eauto.
-  congruence.
-  instantiate (dnum := the_dnum).
-  unfold DIRTREE.find_subtree; simpl; auto.
-  eapply find_name_impl_in_elem; eauto.
-
-  intuition; eauto.
-  repeat (eexists).
-  src_fn_exists.
-  temp_fn_exists.
-
-  instantiate (pathname0 := [temp_fn]).
-  instantiate (bytes1 := bytes').
-  instantiate (attr1 := BYTEFILE.attr0).
-  eauto.
-  rewrite H19.
-  rewrite dirtree_find_update_dents; eauto.
-  eapply find_name_impl_in_elem; eauto.
-
-  eapply pimpl_ok2. eauto with prog. cancel.
-  
-  eapply pimpl_or_r. left.
-  eapply sep_star_lift_r_prop; eauto.
+  eapply pimpl_or_r; right.
   cancel.
-  rewrite find_name_elem_update_exists; auto.
-  eapply find_name_impl_in_elem; eauto.  
 
-  cancel.
-  eapply pimpl_or_r. right.
-  cancel.
-  
+  erewrite update_update_subtree_eq.
   assert (bytes = bytes').
   apply bytes_dst_src_eq with (a := a) (Fx := Fx); eauto.
   rewrite H; auto.
-  rewrite dirtree_update_update_dents; auto.
+  eauto.
 
-  crash_prolog.
-  instantiate( m'0 := m').
-  crash_epilog.
-  instantiate (tinum := temp_inum).
-  rewrite H7; eauto.
-  repeat (eexists).
-  rewrite dirtree_update_update_dents; auto.
-  eapply find_subtree_fold_right_update_ne; auto.
+  cancel.
+  right.
+  pred_apply.
+  apply pimpl_or_r; right.
+  repeat (apply pimpl_exists_r; eexists).
+  instantiate (x := m').
+  instantiate (x0 :=  (DIRTREE.update_subtree [tfn]
+                                              (DIRTREE.TreeFile tinum bytes' BYTEFILE.attr0) temp_tree)).
+  instantiate (x1 := bytes').
+  (* instantiate (x2 := BYTEFILE.attr0). *)
+  cancel.
+  eapply LOG.would_recover_either_pred_ppimpl.
+  apply pimpl_exists_l; intro.
+  repeat (apply pimpl_exists_r; eexists).
+  instantiate (x := x).
+  instantiate (x0 := bytes').
+  instantiate (x1 := attr).
+  cancel.
+  erewrite update_update_subtree_eq in H7.
+  rewrite <- H7; auto.
 
-  src_fn_exists_tree.
-
-  rewrite dirtree_update_update_dents; auto.
-  rewrite find_name_elem_update_exists; auto.
-  eapply find_name_impl_in_elem; auto.
-  temp_fn_exists.
-  intuition; eauto.
-  repeat (eexists).
-
-  eapply find_subtree_fold_right_update_ne; auto.
-  src_fn_exists_tree.
-  erewrite find_name_elem_update_exists; auto.
-  eapply find_name_impl_in_elem; eauto.
-
-  crash_prolog.
-  instantiate (m' := m).
-  crash_epilog.
-  instantiate (tinum := temp_inum).
-  rewrite H14.
-  rewrite find_name_elem_update_exists; eauto.
-  repeat (eexists).
-
-  eapply find_subtree_fold_right_update_ne; auto.
-  src_fn_exists_tree.
-  eapply find_name_impl_in_elem; eauto.
-  intuition; eauto.  
-
-  crush_exists_crash.
-
-  crush_would_recover_either tree_elem.
-  crush_exists_crash.
-
-  crush_would_recover_either tree_elem.
-  crush_exists_crash.
-
-  crush_would_recover_either tree_elem.
-  crush_exists_crash.
+  cancel.
+  right.
+  pred_apply.
+  apply pimpl_or_r; left.
+  eapply LOG.would_recover_either_pred_ppimpl.
+  repeat (apply pimpl_exists_l; intro).
+  cancel.
+  eauto.
   
+  left; auto.
+  left; auto.
+  left; auto.
+Qed.
+
+
+Hint Extern 1 ({{_}} progseq (copy2temp _ _ _ _) _) => apply copy2temp_ok : prog.
+
+(* The file system may crash during a transaction while running atomic_cp or
+atomic_cp_recover. The state of the file system after a crash can be described
+by the following 4 generic states and 6 type of transactions between those 3
+states: *)
+
+Definition temp_fn := ".temp"%string.
+
+
+Inductive state :=
+| UnChanged
+| NoTempFile
+| TempFileExists
+| DstFileExists
+.
+
+Inductive transition :=
+| UnChanged2UnChanged
+| Unchanged2Temp
+| Temp2NoTemp
+| Temp2Temp
+| Temp2Dst
+| Dst2Dst
+.
+
+Definition rep_src_tree src_tree src_dents src_fn dst_fn :=
+  src_fn <> temp_fn /\
+  dst_fn <> temp_fn /\
+  src_fn <> dst_fn  /\
+  rep_root src_tree src_dents /\
+  DIRTREE.find_name [temp_fn] src_tree = None.
+
+(* maybe use update_subtree and prune? *)
+Definition rep_tree st src_tree src_dents (tree: DIRTREE.dirtree) src_fn dst_fn temp_fn :=
+  rep_src_tree src_tree src_dents src_fn dst_fn /\
+  (match st with
+    | UnChanged => tree = src_tree
+    | NoTempFile =>
+      exists telem,
+         tree = DIRTREE.delete_from_dir temp_fn
+                    (DIRTREE.tree_graft the_dnum src_dents [] temp_fn telem src_tree)
+    | TempFileExists =>
+      exists telem,
+        tree = DIRTREE.tree_graft the_dnum src_dents [] temp_fn telem src_tree /\
+        DIRTREE.find_subtree [temp_fn] tree = Some(telem)
+    | DstFileExists =>
+      exists srcinum tinum bytes attr,
+        temp_fn <> src_fn /\ dst_fn <> src_fn /\
+        DIRTREE.find_subtree [src_fn] src_tree = Some (DIRTREE.TreeFile srcinum bytes attr) /\
+        tree = DIRTREE.tree_graft the_dnum src_dents [] dst_fn (DIRTREE.TreeFile tinum bytes attr) src_tree /\
+        DIRTREE.find_subtree [dst_fn] tree = Some (DIRTREE.TreeFile tinum bytes attr) /\
+        DIRTREE.find_name [temp_fn] tree = None
+  end).
+
+Definition rep_crash (t : transition) Fm Ftop fsxp src_tree src_dents src_fn dst_fn :=
+  (match t with
+     | UnChanged2UnChanged =>
+       exists m,
+         [[(Fm * DIRTREE.rep fsxp Ftop src_tree)%pred (list2mem m) ]] *
+         [[rep_tree UnChanged src_tree src_dents src_tree src_fn dst_fn temp_fn ]] *
+         LOG.would_recover_either (FSXPLog fsxp) (sb_rep fsxp) m m
+     | Unchanged2Temp =>
+       exists m,
+        [[(Fm * DIRTREE.rep fsxp Ftop src_tree)%pred (list2mem m) ]] *
+         [[rep_tree UnChanged src_tree src_dents src_tree src_fn dst_fn temp_fn ]] *
+         LOG.would_recover_either_pred (FSXPLog fsxp) (sb_rep fsxp) m
+             (exists tree'',
+                       (Fm * DIRTREE.rep fsxp Ftop tree'') * 
+                       [[rep_tree TempFileExists src_tree src_dents tree'' src_fn dst_fn temp_fn]])
+     | Temp2NoTemp =>
+       exists m' tree',
+         [[ (Fm * DIRTREE.rep fsxp Ftop tree')%pred (list2mem m') ]] *
+         [[rep_tree TempFileExists src_tree src_dents tree' src_fn dst_fn temp_fn ]] *
+         LOG.would_recover_either_pred (FSXPLog fsxp) (sb_rep fsxp) m'
+             (exists tree'',
+                       (Fm * DIRTREE.rep fsxp Ftop tree'') * 
+                       [[rep_tree NoTempFile src_tree src_dents tree'' src_fn dst_fn temp_fn ]])
+     | Temp2Temp =>
+       exists m' tree',
+        [[ (Fm * DIRTREE.rep fsxp Ftop tree')%pred (list2mem m') ]] *
+        [[rep_tree TempFileExists src_tree src_dents tree' src_fn dst_fn temp_fn ]] *
+        LOG.would_recover_either_pred (FSXPLog fsxp) (sb_rep fsxp) m'
+           (exists tree'',
+              (Fm * DIRTREE.rep fsxp Ftop tree'') *
+              [[rep_tree TempFileExists src_tree src_dents tree'' src_fn dst_fn temp_fn ]])
+     | Temp2Dst =>
+       exists m' tree',
+        [[ (Fm * DIRTREE.rep fsxp Ftop tree')%pred (list2mem m') ]] *
+        [[rep_tree TempFileExists src_tree src_dents tree' src_fn dst_fn temp_fn ]] *
+        LOG.would_recover_either_pred (FSXPLog fsxp) (sb_rep fsxp) m'
+            (exists tree'',
+                        (Fm * DIRTREE.rep fsxp Ftop tree'') * 
+                        [[rep_tree DstFileExists src_tree src_dents tree'' src_fn dst_fn temp_fn ]])
+     | Dst2Dst =>
+       exists m' tree',
+        [[ (Fm * DIRTREE.rep fsxp Ftop tree')%pred (list2mem m') ]] *
+        [[rep_tree DstFileExists src_tree src_dents tree' src_fn dst_fn temp_fn ]] *
+        LOG.would_recover_either_pred (FSXPLog fsxp) (sb_rep fsxp) m'
+            (exists tree'',
+                        (Fm * DIRTREE.rep fsxp Ftop tree'') * 
+                        [[rep_tree DstFileExists src_tree src_dents tree'' src_fn dst_fn temp_fn ]])
+
+   end)%pred.
+
+Definition tree_reps src_tree src_dents cur_tree src_fn dst_fn   :=
+  rep_tree UnChanged src_tree src_dents cur_tree src_fn dst_fn temp_fn  \/
+  rep_tree NoTempFile src_tree src_dents cur_tree src_fn dst_fn temp_fn  \/
+  rep_tree TempFileExists src_tree src_dents cur_tree src_fn dst_fn temp_fn  \/
+  rep_tree DstFileExists src_tree src_dents cur_tree src_fn dst_fn temp_fn .
+
+Definition crash_transitions Fm Ftop fsxp src_tree src_dents src_fn dst_fn  :=
+  (rep_crash UnChanged2UnChanged Fm Ftop fsxp src_tree src_dents src_fn dst_fn  \/
+   rep_crash Unchanged2Temp Fm Ftop fsxp src_tree src_dents src_fn dst_fn  \/
+   rep_crash Temp2NoTemp Fm Ftop fsxp src_tree src_dents src_fn dst_fn  \/
+   rep_crash Temp2Temp Fm Ftop fsxp src_tree src_dents src_fn dst_fn  \/
+   rep_crash Temp2Dst Fm Ftop fsxp src_tree src_dents src_fn dst_fn \/
+   rep_crash Dst2Dst Fm Ftop fsxp src_tree src_dents src_fn dst_fn )%pred.
+
+Definition TempTree_rep src_dents telem :=
+  (DIRTREE.tree_graft the_dnum src_dents [] temp_fn telem  (DIRTREE.TreeDir the_dnum src_dents)).
+
+Definition TempTree_mem Fm Ftop fsxp m' src_dents telem :=
+  (Fm * DIRTREE.rep fsxp Ftop  (TempTree_rep src_dents telem))%pred (list2mem m').
+
+Lemma TempFileExists_ok: forall src_tree src_dents src_fn dst_fn telem,
+  rep_src_tree src_tree src_dents src_fn dst_fn ->
+  rep_tree TempFileExists (DIRTREE.TreeDir the_dnum src_dents) src_dents
+           (TempTree_rep src_dents telem) src_fn dst_fn temp_fn.
+Proof.
+  unfold TempTree_rep, rep_tree, rep_src_tree, rep_root; intros.
+  intuition.
+  subst src_tree.
+  eauto.
+  exists telem.
+  split.
+  eauto.
+  rewrite find_subtree_graft_dents; eauto.
+Qed.
+
+Definition DstFileTree_rep src_dents dst_fn tinum bytes attr :=
+  (DIRTREE.tree_graft the_dnum src_dents [] dst_fn
+                      (DIRTREE.TreeFile tinum bytes attr)
+                      (DIRTREE.TreeDir the_dnum src_dents)).
+
+Lemma DstFileExists_ok: forall src_tree src_dents src_fn dst_fn src_inum tinum bytes attr,
+  rep_src_tree src_tree src_dents src_fn dst_fn ->
+  DIRTREE.find_subtree [src_fn] (DIRTREE.TreeDir the_dnum src_dents) =
+            Some (DIRTREE.TreeFile src_inum bytes attr) ->
+  rep_tree DstFileExists (DIRTREE.TreeDir the_dnum src_dents) src_dents
+           (DstFileTree_rep src_dents dst_fn tinum bytes attr) src_fn dst_fn temp_fn.
+Proof.
+  unfold rep_tree, rep_src_tree, rep_root; intros.
+  intuition.
+  subst src_tree; eauto.
+  subst src_tree.
+  eauto.
+  exists src_inum.
+  exists tinum.
+  exists bytes.
+  exists attr.
+  unfold DstFileTree_rep.
+  repeat (rewrite graft_root_is_add_root_dents).
+  rewrite find_subtree_add_root_dents.
+  intuition; eauto.
+  rewrite find_name_add_root_dents_ne; eauto.
+Qed.
+
+
+Lemma temp_impl_Temp2Temp: forall Fm fsxp Ftop m src_tree src_dents src_fn dst_fn tinum bytes attr,
+  rep_src_tree src_tree src_dents src_fn dst_fn ->
+  TempTree_mem Fm Ftop fsxp m src_dents (DIRTREE.TreeFile tinum bytes attr)  ->
+  LOG.would_recover_either (FSXPLog fsxp) (sb_rep fsxp) m m =p=>
+  crash_transitions Fm Ftop fsxp (DIRTREE.TreeDir the_dnum src_dents) src_dents src_fn dst_fn.
+Proof.
+  intros.
+  unfold crash_transitions.
+  unfold TempTree_mem in H0.
+  apply pimpl_or_r; right.
+  apply pimpl_or_r; right.
+  apply pimpl_or_r; right.
+  apply pimpl_or_r; left.
+  unfold rep_crash.
+  exists m.
+  exists (DIRTREE.tree_graft the_dnum src_dents [] temp_fn
+            (DIRTREE.TreeFile tinum bytes attr)
+            (DIRTREE.TreeDir the_dnum src_dents)).
+  pred_apply.
+  cancel.
+  apply would_recover_either_pimpl_pred.
+  exists  (DIRTREE.tree_graft the_dnum src_dents [] temp_fn
+            (DIRTREE.TreeFile tinum bytes attr)
+            (DIRTREE.TreeDir the_dnum src_dents)).
+  pred_apply.
+  cancel.
+  eapply TempFileExists_ok; eauto.
+  eapply TempFileExists_ok; eauto.
+Qed.
+
+
+Lemma temp_impl_pred_Temp2Temp: forall Fm fsxp Ftop m src_tree src_dents src_fn dst_fn tinum pred bytes attr,
+  rep_src_tree src_tree src_dents src_fn dst_fn ->
+  TempTree_mem Fm Ftop fsxp m src_dents (DIRTREE.TreeFile tinum bytes attr) ->
+  pred = (exists
+        (tree' : DIRTREE.dirtree) (b : list Bytes.byte) 
+      (a : BYTEFILE.bytefile_attr),
+        Fm * DIRTREE.rep fsxp Ftop tree' *
+        [[tree' =
+          DIRTREE.update_subtree [temp_fn] (DIRTREE.TreeFile tinum b a)
+            (DIRTREE.tree_graft the_dnum src_dents [] temp_fn
+               (DIRTREE.TreeFile tinum [] BYTEFILE.attr0)
+               (DIRTREE.TreeDir the_dnum src_dents))]])%pred ->
+  LOG.would_recover_either_pred (FSXPLog fsxp) (sb_rep fsxp) m pred  =p=>
+   crash_transitions Fm Ftop fsxp (DIRTREE.TreeDir the_dnum src_dents) src_dents src_fn dst_fn.
+Proof.
+  intros.
+  unfold crash_transitions.
+  apply pimpl_or_r; right.
+  apply pimpl_or_r; right.
+  apply pimpl_or_r; right.
+  apply pimpl_or_r; left.
+  unfold rep_crash.
+  exists m.
+  subst pred.
+  pred_apply.
+  cancel.
+  eapply LOG.would_recover_either_pred_ppimpl.
+  repeat (apply pimpl_exists_l; intro).
+  cancel.
+  subst x.
+  rewrite update_subtree_graft_dents.
+  eapply TempFileExists_ok; eauto.
+  unfold rep_src_tree, rep_root in H.
+  intuition.
+  subst src_tree.
+  eauto.
+  unfold TempTree_mem in H0.
+  pred_apply.
+  cancel.
+  eapply TempFileExists_ok; eauto.
+Qed.
+
+(* XXX this rep should be defined in from FS.v *)
+Definition rename_return_rep Fm Ftop fsxp src_dents dst_fn tinum attr bytes :=
+  let temp_dents := (DIRTREE.add_to_list temp_fn
+                                         (DIRTREE.TreeFile tinum bytes attr) src_dents) in
+   (exists
+       (srcnum : addr) (srcents : list (string * DIRTREE.dirtree)) 
+       (dstnum : addr) (dstents : list (string * DIRTREE.dirtree)) 
+       (subtree pruned renamed tree' : DIRTREE.dirtree),
+       Fm * DIRTREE.rep fsxp Ftop tree' *
+       [[DIRTREE.find_subtree [] (DIRTREE.TreeDir the_dnum temp_dents) =
+         Some (DIRTREE.TreeDir srcnum srcents)]] *
+       [[DIRTREE.find_dirlist temp_fn srcents = Some subtree]] *
+       [[pruned = DIRTREE.tree_prune srcnum srcents [] temp_fn
+                            (DIRTREE.TreeDir the_dnum temp_dents)]] *
+       [[DIRTREE.find_subtree [] pruned = Some (DIRTREE.TreeDir dstnum dstents)]] *
+       [[renamed = DIRTREE.tree_graft dstnum dstents [] dst_fn subtree pruned]] *
+       [[tree' =
+          DIRTREE.update_subtree [] renamed
+            (DIRTREE.update_subtree [temp_fn]
+               (DIRTREE.TreeFile tinum bytes attr)
+               (DIRTREE.tree_graft the_dnum src_dents [] temp_fn
+                  (DIRTREE.TreeFile tinum [] BYTEFILE.attr0)
+                  (DIRTREE.TreeDir the_dnum src_dents)))]])%pred.
+
+Lemma rename_return_rep_impl_DstFileExists: forall Fm Ftop fsxp src_tree src_dents src_fn src_inum dst_fn tinum bytes attr,
+  rep_src_tree src_tree src_dents src_fn dst_fn ->
+  DIRTREE.find_subtree [src_fn] (DIRTREE.TreeDir the_dnum src_dents) =
+            Some (DIRTREE.TreeFile src_inum bytes attr) ->
+  rename_return_rep Fm Ftop fsxp src_dents dst_fn tinum attr bytes =p=>
+  (exists tree'' : DIRTREE.dirtree,
+      Fm * DIRTREE.rep fsxp Ftop tree'' *
+      [[rep_tree DstFileExists (DIRTREE.TreeDir the_dnum src_dents) src_dents
+          tree'' src_fn dst_fn temp_fn]]).
+Proof.
+  unfold rename_return_rep; intros.
+  eexists (DstFileTree_rep src_dents dst_fn tinum bytes attr).
+  unfold DstFileTree_rep.
+  pred_apply.
+  cancel.
+  rewrite update_subtree_root.
+  rewrite find_root_finds_root in H9.
+  inversion H9.
+  subst srcents.
+  subst srcnum.
+  rewrite prune_add_root_dents.
+  rewrite find_dirlist_add_dents in H8.
+  inversion H8.
+  subst subtree.
+  (* rework H4 *)
+  admit.
+  eapply DstFileExists_ok; eauto.
+Admitted.
+
+Lemma temp_rename_impl_Temp2Dst: forall Fm fsxp Ftop m' src_tree src_dents src_fn src_inum dst_fn tinum bytes attr,
+  rep_src_tree src_tree src_dents src_fn dst_fn ->
+  DIRTREE.find_subtree [src_fn] (DIRTREE.TreeDir the_dnum src_dents) =
+           Some (DIRTREE.TreeFile src_inum bytes attr) ->
+  TempTree_mem Fm Ftop fsxp m' src_dents (DIRTREE.TreeFile tinum bytes attr) ->
+  LOG.would_recover_either_pred (FSXPLog fsxp) (sb_rep fsxp) m'
+     (rename_return_rep Fm Ftop fsxp src_dents dst_fn tinum attr bytes) =p=>
+  crash_transitions Fm Ftop fsxp (DIRTREE.TreeDir the_dnum src_dents) src_dents src_fn dst_fn.
+Proof.
+  intros.
+  unfold crash_transitions.
+  apply pimpl_or_r; right.
+  apply pimpl_or_r; right.
+  apply pimpl_or_r; right.
+  apply pimpl_or_r; right.
+  apply pimpl_or_r; left.
+  unfold rep_crash.
+  exists m'.
+  exists (DIRTREE.tree_graft the_dnum src_dents [] temp_fn
+                (DIRTREE.TreeFile tinum bytes attr)
+                (DIRTREE.TreeDir the_dnum src_dents)).
+  pred_apply.
+  cancel.
+  eapply LOG.would_recover_either_pred_ppimpl.
+  eapply rename_return_rep_impl_DstFileExists; eauto.
+  eapply TempFileExists_ok; eauto.
+Qed.
+
+Definition NoTempTree_rep src_dents telem :=
+  (DIRTREE.delete_from_dir temp_fn (DIRTREE.TreeDir the_dnum (DIRTREE.add_to_list temp_fn telem src_dents))).
+
+Lemma NoTemp_ok: forall src_tree src_dents src_fn dst_fn telem,
+  rep_src_tree src_tree src_dents src_fn dst_fn ->
+  rep_tree NoTempFile (DIRTREE.TreeDir the_dnum src_dents) src_dents
+           (NoTempTree_rep src_dents telem) src_fn dst_fn temp_fn.
+Proof.
+  unfold NoTempTree_rep, rep_tree, rep_src_tree, rep_root; intros.
+  intuition.
+  subst src_tree.
+  eauto.
+  exists telem.
+  rewrite graft_root_is_add_root_dents; eauto.
+Qed.
+
+Lemma TempFileExists_impl_Temp2NoTemp: forall Fm fsxp Ftop m src_tree src_dents src_fn dst_fn tinum pred bytes attr tree',
+  rep_src_tree src_tree src_dents src_fn dst_fn ->
+  (Fm * DIRTREE.rep fsxp Ftop tree')%pred (list2mem m) ->
+  rep_tree TempFileExists src_tree src_dents tree' src_fn dst_fn temp_fn ->
+  pred = (exists tree'' : DIRTREE.dirtree,
+        Fm * DIRTREE.rep fsxp Ftop tree'' *
+        [[tree'' =
+          (DIRTREE.delete_from_dir temp_fn
+               (DIRTREE.TreeDir the_dnum
+                  (DIRTREE.add_to_list temp_fn
+                     (DIRTREE.TreeFile tinum bytes attr) src_dents)))]])%pred ->
+  LOG.would_recover_either_pred (FSXPLog fsxp) (sb_rep fsxp) m pred =p=>
+  crash_transitions Fm Ftop fsxp (DIRTREE.TreeDir the_dnum src_dents) src_dents src_fn dst_fn.
+Proof.
+  unfold rep_src_tree, rep_root, crash_transitions; intros.
+  apply pimpl_or_r; right.
+  apply pimpl_or_r; right.
+  apply pimpl_or_r; left.
+  unfold rep_crash.
+  exists m.
+  exists tree'.
+  pred_apply.
+  cancel.
+  eapply LOG.would_recover_either_pred_ppimpl.
+  repeat (apply pimpl_exists_l; intro).
+  cancel.
+  subst x.
+  eapply NoTemp_ok; eauto.
+  unfold rep_src_tree; intuition; eauto.
+  unfold rep_root; eauto.
+Qed.
+
+Lemma UnChanged_ok: forall src_tree src_dents src_fn dst_fn,
+  rep_src_tree src_tree src_dents src_fn dst_fn ->
+  rep_tree UnChanged src_tree src_dents src_tree src_fn dst_fn temp_fn.
+Proof.
+  unfold rep_tree, rep_src_tree, rep_root; intros.
+  intuition; eauto.
+Qed.
+
+
+Lemma newtemp_impl_UnChanged2Temp: forall Fm fsxp Ftop m src_tree src_dents src_fn dst_fn pred,
+  rep_src_tree src_tree src_dents src_fn dst_fn ->
+  (Fm * DIRTREE.rep fsxp Ftop src_tree)%pred (list2mem m) ->
+  pred = (exists (inum : addr) (tree' : DIRTREE.dirtree),
+      Fm * DIRTREE.rep fsxp Ftop tree' *
+      [[tree' = DIRTREE.tree_graft the_dnum src_dents [] temp_fn 
+         (DIRTREE.TreeFile inum [] BYTEFILE.attr0) src_tree]])%pred ->
+  LOG.would_recover_either_pred (FSXPLog fsxp) (sb_rep fsxp) m pred  =p=>
+   crash_transitions Fm Ftop fsxp (DIRTREE.TreeDir the_dnum src_dents) src_dents src_fn dst_fn.
+Proof.
+  intros.
+  unfold crash_transitions.
+  apply pimpl_or_r; right.
+  apply pimpl_or_r; left.
+  unfold rep_crash.
+  exists m.
+  subst pred.
+  pred_apply.
+  cancel.
+  eapply LOG.would_recover_either_pred_ppimpl.
+  repeat (apply pimpl_exists_l; intro).
+  cancel.
+  subst x0.
+  unfold rep_src_tree, rep_root in H.
+  intuition.
+  subst src_tree.
+  eapply TempFileExists_ok; eauto.
+  unfold rep_src_tree, rep_root; eauto.
+  unfold rep_src_tree, rep_root in H.
+  intuition.
+  subst src_tree.
+  cancel.
+  unfold rep_tree.
+  intuition.
+  unfold rep_src_tree, rep_root; eauto.
+  unfold rep_src_tree, rep_root in H.
+  intuition.
+  subst src_tree; eauto.
+Qed.
+
+Lemma unchanged_impl_UnChanged2UnChanged: forall Fm fsxp Ftop m src_tree src_dents src_fn dst_fn,
+  rep_src_tree src_tree src_dents src_fn dst_fn ->
+  (Fm * DIRTREE.rep fsxp Ftop src_tree)%pred (list2mem m) ->
+  LOG.would_recover_either (FSXPLog fsxp) (sb_rep fsxp) m m  =p=>
+  crash_transitions Fm Ftop fsxp src_tree src_dents src_fn dst_fn.
+Proof.
+  intros.
+  unfold crash_transitions.
+  apply pimpl_or_r; left.
+  unfold rep_crash.
+  exists m.
+  pred_apply.
+  cancel.
+  unfold rep_tree; eauto.
+Qed.
+
+
+Definition atomic_cp_return_rep_ok  src_tree src_dents dst_tree src_fn dst_fn :=
+  rep_tree DstFileExists src_tree src_dents dst_tree src_fn dst_fn temp_fn.
+
+Definition copy_and_rename_rep_nok src_tree src_dents tree' src_fn dst_fn :=
+  rep_tree TempFileExists src_tree src_dents tree' src_fn dst_fn temp_fn.
+
+Definition copy_and_rename_rep fsxp Fm Ftop src_tree src_dents src_fn dst_fn mscs r :=
+  (exists m' tree',
+    LOG.rep (FSXPLog fsxp) (sb_rep fsxp) (NoTransaction m') mscs *
+    [[ (Fm * DIRTREE.rep fsxp Ftop tree')%pred (list2mem m') ]] *
+    (([[ r = false ]] * [[ copy_and_rename_rep_nok src_tree src_dents tree' src_fn dst_fn ]]) \/
+     ([[ r = true ]] * [[ atomic_cp_return_rep_ok src_tree src_dents tree' src_fn dst_fn ]]))
+     )%pred.
+
+Definition copy_and_rename T fsxp src_inum dst_inum dst_fn mscs rx : prog T :=
+  let^ (mscs, ok) <- copy2temp fsxp src_inum dst_inum mscs;
+  match ok with
+    | false =>
+        rx ^(mscs, false)
+    | true =>
+      let^ (mscs, ok1) <- FS.rename fsxp the_dnum [] temp_fn [] dst_fn mscs;
+      rx ^(mscs, ok1)
+  end.
+
+Theorem copy_and_rename_ok : forall fsxp src_inum tinum dst_fn mscs,
+  {< m Fm Ftop src_tree src_dents temp_tree src_fn bytes attr,
+  PRE   LOG.rep (FSXPLog fsxp) (sb_rep fsxp) (NoTransaction m) mscs *
+        [[ (Fm * DIRTREE.rep fsxp Ftop temp_tree)%pred (list2mem m) ]] *
+        [[ rep_src_tree src_tree src_dents src_fn dst_fn ]]  *
+        [[ DIRTREE.find_subtree [src_fn] src_tree =
+           Some (DIRTREE.TreeFile src_inum bytes attr) ]] *
+        [[ temp_tree = TempTree_rep src_dents (DIRTREE.TreeFile tinum [] BYTEFILE.attr0) ]] *
+        [[ DIRTREE.find_subtree [temp_fn] temp_tree =
+           Some (DIRTREE.TreeFile tinum [] BYTEFILE.attr0) ]]
+ POST RET:^(mscs, r)
+   copy_and_rename_rep fsxp Fm Ftop src_tree src_dents src_fn dst_fn mscs r          
+ CRASH
+   crash_transitions Fm Ftop fsxp src_tree src_dents src_fn dst_fn
+>} copy_and_rename fsxp src_inum tinum dst_fn mscs.
+Proof.
+  unfold copy_and_rename, copy_and_rename_rep, atomic_cp_return_rep_ok, copy_and_rename_rep_nok, rep_src_tree, rep_root, TempTree_rep; intros.
+  (* copy2temp *)
+  step.
+  
+  subst src_tree.
+  instantiate (src_fn0 := src_fn).
+  instantiate (bytes0 := bytes).
+  instantiate (attr0 := attr).
+  erewrite find_subtree_graft_dents_ne; eauto.
+  instantiate (tfn := temp_fn).
+  subst src_tree.
+  erewrite find_subtree_graft_dents; eauto.
+
+  (* success, now rename *)
+  step.
+  instantiate (cwd1 := []).
+  erewrite update_subtree_graft_dents.
+  erewrite find_root_graft_dents; eauto.
+  eauto.
+
+  (* return *)
+  step.
+  (* rename failed *)
+  apply pimpl_or_r; left.
+  cancel.
+
+  rewrite update_subtree_graft_dents.
+  eapply TempFileExists_ok with (src_tree := (DIRTREE.TreeDir the_dnum src_dents)); eauto.
+  unfold rep_src_tree, rep_root; eauto.
+  eauto.
+   
+  (* rename succeeded *)
+  apply pimpl_or_r; right.
+  cancel.
+
+  rewrite find_root_add_to_list in H22.
+  inversion H22; subst.
+  rewrite find_dirlist_add_dents in H21.
+  inversion H21; subst subtree.
+  rewrite find_root_prune_add_list in H19.
+  inversion H19.
+  subst dstnum.
+  subst dstents.
+
+  rewrite update_subtree_root.
+  erewrite prune_add_root_dents.
+  eapply DstFileExists_ok; eauto.
+  unfold rep_src_tree, rep_root; eauto.
+
+  eapply temp_rename_impl_Temp2Dst; eauto.
+  unfold rep_src_tree, rep_root; eauto.
+  unfold TempTree_mem.
+  rewrite update_subtree_graft_dents in H.
+  assumption.
+  assumption.
+
+  eapply pimpl_or_r; left.
+  cancel.
+  eapply TempFileExists_ok.
+  unfold rep_src_tree, rep_root; eauto.
+
+  (* copy failed *)
+  apply pimpl_or_r; left.
+  cancel.
+  rewrite update_subtree_graft_dents.
+  eapply TempFileExists_ok.
+  unfold rep_src_tree, rep_root; eauto.
+  eauto.
+
+  eapply temp_impl_Temp2Temp with (bytes := []) (attr := BYTEFILE.attr0); eauto.
+  unfold rep_src_tree, rep_root; eauto.
+
+  eapply temp_impl_pred_Temp2Temp with (bytes := []) (attr := BYTEFILE.attr0); eauto.
+  unfold rep_src_tree, rep_root; eauto.
+
+  eapply temp_impl_pred_Temp2Temp with (m := a) (bytes := a1) (attr := a2); eauto.
+  unfold rep_src_tree, rep_root; eauto.
+  unfold TempTree_mem.
+  pred_apply.
+  subst a0.
+  cancel.
+  erewrite update_subtree_graft_dents.
+  cancel.
+  eauto.  
   Grab Existential Variables.
   all: eauto.
 Qed.
 
 
-Hint Extern 1 ({{_}} progseq (copy2temp _ _ _ _) _) => apply copy2temp_ok : prog.
+Definition atomic_cp_return_rep_nok src_tree src_dents tree' src_fn dst_fn :=
+  rep_tree UnChanged src_tree src_dents tree' src_fn dst_fn temp_fn \/
+  rep_tree NoTempFile src_tree src_dents tree' src_fn dst_fn temp_fn.
+
+Definition atomic_cp_return_rep fsxp Fm Ftop src_tree src_dents src_fn dst_fn mscs r :=
+  (exists m' tree',
+    LOG.rep (FSXPLog fsxp) (sb_rep fsxp) (NoTransaction m') mscs *
+    [[ (Fm * DIRTREE.rep fsxp Ftop tree')%pred (list2mem m') ]] *
+    (([[ r = false ]] * [[ atomic_cp_return_rep_nok src_tree src_dents tree' src_fn dst_fn ]]) \/
+     ([[ r = true ]] * [[ atomic_cp_return_rep_ok src_tree src_dents tree' src_fn dst_fn ]]))
+     )%pred.
+
+Definition copy_and_rename_cleanup T fsxp src_inum dst_inum dst_fn mscs rx : prog T :=
+  let^ (mscs, ok) <- copy_and_rename fsxp src_inum dst_inum dst_fn mscs;
+  match ok with
+    | false =>
+      let^ (mscs, ok) <- FS.delete fsxp the_dnum temp_fn mscs;
+      (* What if FS.delete fails?? *)
+      rx ^(mscs, false)
+    | true =>
+      rx ^(mscs, true)
+  end.
+
+Hint Extern 1 ({{_}} progseq (copy_and_rename _ _ _ _ _) _) => apply copy_and_rename_ok : prog.
+
+Theorem copy_and_rename_cleanup_ok : forall fsxp src_inum tinum dst_fn mscs,
+  {< m Fm Ftop src_tree src_dents temp_tree src_fn bytes attr,
+  PRE   LOG.rep (FSXPLog fsxp) (sb_rep fsxp) (NoTransaction m) mscs *
+        [[ (Fm * DIRTREE.rep fsxp Ftop temp_tree)%pred (list2mem m) ]] *
+        [[ rep_src_tree src_tree src_dents src_fn dst_fn ]]  *
+        [[ DIRTREE.find_subtree [src_fn] src_tree =
+           Some (DIRTREE.TreeFile src_inum bytes attr) ]] *
+        [[ temp_tree = TempTree_rep src_dents (DIRTREE.TreeFile tinum [] BYTEFILE.attr0) ]] *
+        [[ DIRTREE.find_subtree [temp_fn] temp_tree =
+           Some (DIRTREE.TreeFile tinum [] BYTEFILE.attr0) ]]
+ POST RET:^(mscs, r)
+   atomic_cp_return_rep fsxp Fm Ftop src_tree src_dents src_fn dst_fn mscs r          
+ CRASH
+   crash_transitions Fm Ftop fsxp src_tree src_dents src_fn dst_fn
+>} copy_and_rename_cleanup fsxp src_inum tinum dst_fn mscs.
+Proof.
+  unfold copy_and_rename_cleanup, atomic_cp_return_rep; intros.
+  step.
+  destruct a.
+  eapply pimpl_ok2.
+  eauto with prog.
+  unfold copy_and_rename_rep.
+  cancel.
+  apply pimpl_or_r; right.
+  cancel.
+
+  unfold copy_and_rename_rep.  
+  eapply pimpl_ok2.
+  eauto with prog.
+  cancel.
+  instantiate (pathname := []).
+  unfold copy_and_rename_rep_nok in H13.
+  (* admit: delete failed *)
+  admit.
+
+  step.
+  apply pimpl_or_r; left.
+  cancel.
+  unfold copy_and_rename_rep_nok in H13.
+  unfold atomic_cp_return_rep_nok.
+  (* delete failed *)
+  admit.
+
+  apply pimpl_or_r; left.
+  cancel.
+  unfold atomic_cp_return_rep_nok.
+  right.
+  (* file is deleted *)
+  admit.
+  admit.
+
+  cancel.
+  unfold copy_and_rename_rep_nok in H13.
+  instantiate (tree_elem := DIRTREE.add_to_list temp_fn
+                                         (DIRTREE.TreeFile tinum bytes attr) src_dents).
+
+  erewrite update_subtree_root.
+  unfold rep_src_tree, rep_root in H7.
+  intuition.
+  subst src_tree.
+  eapply TempFileExists_impl_Temp2NoTemp with (m := m'); eauto.
+  unfold rep_src_tree, rep_root; eauto.
+  Unshelve.
+  all: eauto.
+Admitted.
+
+Hint Extern 1 ({{_}} progseq (copy_and_rename_cleanup _ _ _ _ _) _) => apply copy_and_rename_cleanup_ok : prog.
+
+Definition atomic_cp_src T fsxp src_inum dst_fn mscs rx : prog T :=
+  let^ (mscs, maybe_dst_inum) <- FS.create fsxp the_dnum temp_fn mscs;
+  match maybe_dst_inum with
+    | None => rx ^(mscs, false)
+    | Some dst_inum =>
+      let^ (mscs, ok) <- copy_and_rename_cleanup fsxp src_inum dst_inum dst_fn mscs;
+      rx ^(mscs, ok)
+  end.
+
+Theorem atomic_cp_src_ok : forall fsxp src_inum bytes attr dst_fn mscs,
+  {< m Fm Ftop src_tree src_dents src_fn,
+  PRE   LOG.rep (FSXPLog fsxp) (sb_rep fsxp) (NoTransaction m) mscs *
+        [[ (Fm * DIRTREE.rep fsxp Ftop src_tree)%pred (list2mem m) ]] *
+        [[ rep_src_tree src_tree src_dents src_fn dst_fn ]] *
+        [[ DIRTREE.find_subtree [src_fn] src_tree =
+           Some (DIRTREE.TreeFile src_inum bytes attr) ]]
+  POST RET:^(mscs, r)
+    atomic_cp_return_rep fsxp Fm Ftop src_tree src_dents src_fn dst_fn mscs r
+  CRASH
+    crash_transitions Fm Ftop fsxp src_tree src_dents src_fn dst_fn
+  >} atomic_cp_src fsxp src_inum dst_fn mscs.
+Proof.
+  unfold atomic_cp_src, atomic_cp_return_rep; intros.
+  step.
+  instantiate (pathname := []).
+  instantiate (tree_elem := src_dents).
+  unfold rep_src_tree, rep_root in H5.
+  intuition.
+  subst src_tree; eauto.
+  step.
+  unfold TempTree_rep.
+  rewrite find_subtree_graft_dents; eauto.
+  step.
+  apply pimpl_or_r; left.
+  cancel.
+  unfold atomic_cp_return_rep_nok.
+  left. unfold rep_tree.
+  unfold rep_src_tree, rep_root; eauto.
+  unfold rep_src_tree, rep_root in H5.
+  intuition.
+  subst src_tree.
+  eapply newtemp_impl_UnChanged2Temp; eauto.
+  unfold rep_src_tree, rep_root; eauto.
+  Unshelve.
+  all: eauto.
+Qed.
+
+Hint Extern 1 ({{_}} progseq (atomic_cp_src _ _ _ _) _) => apply atomic_cp_src_ok : prog.
 
 Definition atomic_cp T fsxp src_fn dst_fn mscs rx : prog T :=
   let^ (mscs, maybe_src_inum) <- FS.lookup fsxp the_dnum [src_fn] mscs;
@@ -911,246 +1588,50 @@ Definition atomic_cp T fsxp src_fn dst_fn mscs rx : prog T :=
     If (bool_dec isdir true) {
       rx ^(mscs, false)
     } else {
-      let^ (mscs, maybe_dst_inum) <- FS.create fsxp the_dnum temp_fn mscs;
-      match maybe_dst_inum with
-      | None => rx ^(mscs, false)
-      | Some dst_inum =>
-        let^ (mscs, ok) <- copy2temp fsxp src_inum dst_inum mscs;
-        match ok with
-        | false =>
-          let^ (mscs, ok) <- FS.delete fsxp the_dnum temp_fn mscs;
-          (* What if FS.delete fails?? *)
-          rx ^(mscs, false)
-        | true =>
-          let^ (mscs, ok) <- FS.rename fsxp the_dnum [] temp_fn [] dst_fn mscs;
-          match ok with
-          | false =>
-            let^ (mscs, ok) <- FS.delete fsxp the_dnum temp_fn mscs;
-            (* What if FS.delete fails?? *)
-            rx ^(mscs, false)
-          | true =>
-            rx ^(mscs, true)
-          end
-        end
-      end
+      let^ (mscs, ok) <- atomic_cp_src fsxp src_inum dst_fn mscs;
+      rx ^(mscs, ok)
     }
   end.
 
-Ltac NoDup :=
-  match goal with
-    | [ H : (_ * DIRTREE.rep _ _ (DIRTREE.TreeDir _ ?list)) %pred _ |- NoDup (map fst ?list) ] => idtac "nodup"; eapply DIRTREE.rep_tree_names_distinct in H; idtac "step 1: " H; eapply tree_names_distinct_nodup in H; assumption
-  end.                            
-
-Definition atomic_cp_return_rep_ok  tree tree_elem tree' src_fn dst_fn :=
-  exists old_inum new_inum bytes attr,
-    DIRTREE.find_name [temp_fn] tree' = None /\
-    DIRTREE.find_subtree [src_fn] tree = Some (DIRTREE.TreeFile old_inum bytes attr) /\
-    tree' = DIRTREE.tree_graft the_dnum tree_elem [] dst_fn (DIRTREE.TreeFile new_inum bytes attr) tree.
-
-Definition atomic_cp_return_rep fsxp Fm Ftop tree tree_elem src_fn dst_fn mscs r :=
-  (exists m' tree',
-    LOG.rep (FSXPLog fsxp) (sb_rep fsxp) (NoTransaction m') mscs *
-    [[ (Fm * DIRTREE.rep fsxp Ftop tree')%pred (list2mem m') ]] *
-    (([[ r = false ]] *
-      [[ DIRTREE.find_name [temp_fn] tree' = None ]]) \/
-     ([[ r = true ]] * [[ atomic_cp_return_rep_ok tree tree_elem tree' src_fn dst_fn ]]))
-     )%pred.
-
-Theorem atomic_cp_ok : forall fsxp src_fn dst_fn mscs,
-  {< m Fm Ftop tree tree_elem,
+Theorem atomic_cp_ok : forall fsxp src_fn dst_fn mscs ,
+  {< m Fm Ftop src_tree src_dents,
   PRE   LOG.rep (FSXPLog fsxp) (sb_rep fsxp) (NoTransaction m) mscs *
-        [[ (Fm * DIRTREE.rep fsxp Ftop tree)%pred (list2mem m) ]] *
-        [[ tree = DIRTREE.TreeDir the_dnum tree_elem ]] *
-        [[ src_fn <> temp_fn ]] *
-        [[ dst_fn <> temp_fn ]] *
-        [[ DIRTREE.find_name [temp_fn] tree = None ]]
- POST RET:^(mscs, r)
-   atomic_cp_return_rep fsxp Fm Ftop tree tree_elem src_fn dst_fn mscs r          
- CRASH
-   crash_transitions Fm Ftop fsxp src_fn dst_fn
->} atomic_cp fsxp src_fn dst_fn mscs.
+        [[ (Fm * DIRTREE.rep fsxp Ftop src_tree)%pred (list2mem m) ]] *
+        [[ rep_src_tree src_tree src_dents src_fn dst_fn ]]
+  POST RET:^(mscs, r)
+    atomic_cp_return_rep fsxp Fm Ftop src_tree src_dents src_fn dst_fn mscs r
+  CRASH
+    crash_transitions Fm Ftop fsxp src_tree src_dents src_fn dst_fn
+  >} atomic_cp fsxp src_fn dst_fn mscs.
 Proof.
-  unfold atomic_cp, atomic_cp_return_rep, atomic_cp_return_rep_ok; intros.
+  unfold atomic_cp, atomic_cp_return_rep, atomic_cp_return_rep_nok, rep_root; intros.
   step.
-  subst; simpl; auto.
-  subst; simpl; auto.
-
-  step.
-  step.
-  step.
-  instantiate (pathname := []).
-  reflexivity.
-
-  edestruct (DIRTREE.find_name_exists) with (path := [src_fn]); intuition eauto.
-  (* [src_fn] points to a file.  destruct [x], consider both cases, one will be false. *)
-  destruct x; try solve [ exfalso; eauto ].
-
-  step. (* file_copy *)
-
-  rewrite dirtree_add_dents_ne.
-  eauto.
+  unfold rep_src_tree, rep_root in H4.
   intuition.
-
-  
-  (* rewrite find_name_add_to_list. *)
-  admit.
-  
-  step. (* rename *)
-  
-  instantiate (cwd := []).
-  simpl. subst. eauto.
-  
-  step. (* return *)
-
-  eapply pimpl_or_r. right.
-  cancel.
-  repeat (eexists); eauto.
-  
-  (* we got rid of the temporary file in the tree *)
-  instantiate (new_inum := inum).
-  rewrite dirtree_update_add_dents.
-  rewrite dirtree_prune_add_dents with (elem := (DIRTREE.TreeFile inum l b1)) (tree_elem := tree_elem).
-
-  (* H17 *)
-  admit.
-  (* H17 *)
-  admit.
-  
-  reflexivity.
-  NoDup.
-  
-  match goal with
-    | [ H: DIRTREE.find_dirlist _ _ = Some ?s |- context[DIRTREE.tree_graft _ _ _ _ ?s] ]  =>
-      rewrite dirtree_update_add_dents in H; [rewrite dirtree_find_add_dents in H; inversion H|idtac "ignore sub"]
-  end.
-                                                
-  match goal with
-    | [ H: DIRTREE.TreeDir _ _ = DIRTREE.tree_prune _ _ _ _ _ |- _ ]  =>
-      rewrite dirtree_update_add_dents in H; [rewrite dirtree_prune_add_dents with (elem :=  (DIRTREE.TreeFile inum l b1)) (tree_elem := tree_elem) in H; inversion H|idtac "ignore sub"]
-  end.
-
-  rewrite dirtree_update_add_dents.
-  rewrite dirtree_prune_add_dents with (elem :=  (DIRTREE.TreeFile inum l b1)) (tree_elem := tree_elem).
-  reflexivity.
-  (* H17 *)
-  admit.
-  reflexivity.
-  
-  NoDup.
-  admit.
-  reflexivity.
-  NoDup.
-  NoDup.
-    
-  rewrite dirtree_update_add_dents.
-  instantiate (pathname0 := []).
-  instantiate (tree_elem0 :=  (DIRTREE.add_to_list temp_fn (DIRTREE.TreeFile inum l b1) tree_elem)).
-  subst; simpl; eauto.
-  NoDup.
-
+  subst src_tree; eauto.
+  unfold rep_src_tree, rep_root in H4.
+  intuition.
+  subst src_tree; eauto.
   step.
-  eapply pimpl_or_r. left.
+  step.
+  apply pimpl_or_r; left.
   cancel.
-  (* delete failed? *)
-  (* XXX delete shouldn't fail, if temp_fn exists. problem with FS.delete spec *)
-  admit.
-
-  (* delete succeeded *)
-  eapply pimpl_or_r. left.
+  left; unfold rep_tree; eauto.
+  step.
+  erewrite find_name_impl_find_subtree; eauto.
+  eapply not_true_is_false in H7.
+  subst b0; eauto.
+  step.
+  apply pimpl_or_r; left.
   cancel.
-  rewrite dirtree_delete_add_dents.
-  rewrite H4; auto.
-  (* true by H4 *)
-  admit.
-
-  (* temp2notemp *)
-  unfold crash_transitions.
-  eapply pimpl_or_r. right.
-  eapply pimpl_or_r. right.
-  eapply pimpl_or_r. left.
-  unfold rep_crash.
-  eapply pimpl_exists_r. eexists.
-  eapply pimpl_exists_r. eexists.
-  instantiate (x := m').
-  instantiate (x0 := (DIRTREE.TreeDir the_dnum
-            (map
-               (DIRTREE.update_subtree_helper
-                  (fun _ : DIRTREE.dirtree => DIRTREE.TreeFile inum l b1)
-                  temp_fn)
-               (DIRTREE.add_to_list temp_fn
-                  (DIRTREE.TreeFile inum [] BYTEFILE.attr0) tree_elem)))).
-  cancel.
-  eapply LOG.would_recover_either_pred_ppimpl.
-  eapply pimpl_exists_l; intro. cancel.
-  rewrite H13.
-  (* find_name of delete *)
-  rewrite dirtree_delete_add_dents.
-  rewrite H4; auto.
-  admit.
-  admit.
-
-  repeat (eexists).
-  erewrite dirtree_update_add_dents.
-  (* src_fn <> temp_fn *)
-  admit.
-  NoDup.
-  admit.
-
-  (* temp2dst *)
-  unfold crash_transitions.
-  eapply pimpl_or_r. right.
-  eapply pimpl_or_r. right.
-  eapply pimpl_or_r. right.
-  eapply pimpl_or_r. right.
-  eapply pimpl_or_r. left.
-  unfold rep_crash.
-  eapply pimpl_exists_r. eexists.
-  eapply pimpl_exists_r. eexists.
-  instantiate (x := m').
-  instantiate (x0 := (DIRTREE.TreeDir the_dnum
-            (map
-               (DIRTREE.update_subtree_helper
-                  (fun _ : DIRTREE.dirtree => DIRTREE.TreeFile inum l b1)
-                  temp_fn)
-               (DIRTREE.add_to_list temp_fn
-                  (DIRTREE.TreeFile inum [] BYTEFILE.attr0) tree_elem)))).
-  cancel.
-  eapply LOG.would_recover_either_pred_ppimpl.
-  repeat (eexists).
-
-  (* other crash conditions ... *)
-  admit.
-  admit.
-  admit.
-  admit.
-  admit.
-  admit.
-  admit.
-
-  unfold crash_transitions.
-  eapply pimpl_or_r. left.
-  unfold rep_crash.
-  eapply pimpl_exists_r. eexists.
-  eapply pimpl_exists_r. eexists.
-  
-  
-  instantiate (x0 := m).
-  instantiate (x :=  (DIRTREE.TreeDir the_dnum tree_elem)).
-  instantiate (x1 := (DIRTREE.TreeDir the_dnum tree_elem)).
-  admit.
-  (*
-  eapply would_recover_either_pimpl_pred. eexists. 
-  eapply sep_star_lift_apply'; eauto.  *)
-  (*
-  match goal with
-      | [ H: ?t = DIRTREE.TreeDir _ _ |- DIRTREE.find_subtree _ ?t = Some _ ] =>
-          rewrite dirtree_update_add_dents in H; [rewrite H | idtac "ignore sub"]
-  end.
-    *)      
-  
-  Grab Existential Variables.
+  left.
+  eapply UnChanged_ok; eauto.
+  unfold rep_src_tree, rep_root in H4.
+  eapply unchanged_impl_UnChanged2UnChanged; eauto.
+  Unshelve.
   all: eauto.
-Admitted.
+  exact BYTEFILE.attr0.
+Qed.
 
 
 Hint Extern 1 ({{_}} progseq (atomic_cp _ _ _ _) _) => apply atomic_cp_ok : prog.
@@ -1170,19 +1651,15 @@ Definition recover' {T} rx : prog T :=
 
 (* Set Printing Implicit. *)
 
+(* blindly delete temp_fn, if it exists *)
 Definition atomic_cp_cleanup {T} fsxp mscs rx : prog T :=
   let^ (mscs, maybe_src_inum) <- FS.lookup fsxp the_dnum [temp_fn] mscs;
   match maybe_src_inum with
   | None => rx mscs
   | Some (src_inum, isdir) =>
-    If (bool_dec isdir true) {
-      rx mscs
-    } else {
-      let^ (mscs, ok) <- FS.delete fsxp the_dnum temp_fn mscs;
-      rx mscs
-    }
+    let^ (mscs, ok) <- FS.delete fsxp the_dnum temp_fn mscs;
+    rx mscs
   end.
-
 
 Definition atomic_cp_recover {T} rx : prog T :=
   let^ (mscs, fsxp) <- FS.recover;
@@ -1190,192 +1667,210 @@ Definition atomic_cp_recover {T} rx : prog T :=
   rx ^(mscs, fsxp).
   
 
-Definition atomic_cp_recover_rep fsxp Fm Ftop src_fn dst_fn mscs :=
-  (exists m' tree tree_elem tree',
+(* maybe just list the 3 cases? UnChanged, NoTemp, or DstFileExists *)
+Definition atomic_cp_recover_rep fsxp Fm Ftop src_tree src_dents src_fn dst_fn mscs :=
+  (exists m' tree',
     LOG.rep (FSXPLog fsxp) (sb_rep fsxp) (NoTransaction m') mscs *
     [[ (Fm * DIRTREE.rep fsxp Ftop tree')%pred (list2mem m') ]] *
-    ([[ DIRTREE.find_name [temp_fn] tree' = None ]] \/ 
-     [[ atomic_cp_return_rep_ok tree tree_elem tree' src_fn dst_fn ]]))%pred.
+    [[ rep_tree UnChanged src_tree src_dents tree' src_fn dst_fn temp_fn \/
+       rep_tree DstFileExists src_tree src_dents tree' src_fn dst_fn temp_fn ]]
+  )%pred.
 
 
-Lemma root_ok : forall tree tree_elem,
-                  DIRTREE.find_subtree [] tree = Some (DIRTREE.TreeDir the_dnum tree_elem) ->
-                  the_dnum = DIRTREE.dirtree_inum tree /\ DIRTREE.dirtree_isdir tree = true.
-Proof.
-  intros.
-  split.
-  unfold DIRTREE.find_subtree in H.
-  assert (tree = (DIRTREE.TreeDir the_dnum tree_elem)).
-  congruence.
-  subst; simpl; auto.
-  unfold DIRTREE.find_subtree in H.
-  assert (tree = (DIRTREE.TreeDir the_dnum tree_elem)).
-  congruence.
-  subst; simpl; auto.
-Qed.
-
-
-Lemma NoTempFile_recover_ok : forall fsxp mscs,
-  {< m Fm Ftop tree dst_fn src_fn,
+Lemma UnChanged_recover_ok : forall fsxp mscs,
+  {< m Fm Ftop src_tree src_dents tree dst_fn src_fn,
    PRE
      LOG.rep (FSXPLog fsxp) (sb_rep fsxp) (NoTransaction m) mscs *
      [[ (Fm * DIRTREE.rep fsxp Ftop tree)%pred (list2mem m) ]] *
-     [[rep_tree NoTempFile tree src_fn dst_fn temp_fn]]
+     [[rep_tree UnChanged src_tree src_dents tree src_fn dst_fn temp_fn]]
    POST RET:mscs
-     atomic_cp_recover_rep fsxp Fm Ftop src_fn dst_fn mscs
+     atomic_cp_recover_rep fsxp Fm Ftop src_tree src_dents src_fn dst_fn mscs
   CRASH
-    crash_transitions Fm Ftop fsxp src_fn dst_fn
+    crash_transitions Fm Ftop fsxp src_tree src_dents src_fn dst_fn
     >} atomic_cp_cleanup fsxp mscs.
 Proof.
-  unfold atomic_cp_cleanup. intros.
+  unfold atomic_cp_cleanup, atomic_cp_recover_rep, rep_tree, rep_src_tree, rep_root; intros.
   step.
-  unfold rep_root in H3.
-  eapply root_ok; eauto.
-  eapply root_ok; eauto.
+  subst tree.
+  subst src_tree; auto.
+  subst tree.
+  subst src_tree; auto.
   step.
-  unfold atomic_cp_recover_rep.
-  repeat (eapply pimpl_exists_r; eexists).
-  instantiate (x := m). cancel.
-  unfold atomic_cp_return_rep_ok.
-  eapply pimpl_or_r. left.
-  cancel.
+  eapply unchanged_impl_UnChanged2UnChanged; eauto.
+  unfold rep_src_tree, rep_root; eauto.
+  Grab Existential Variables.
+  all: eauto.
+  (* XXX DIRTREE.dirtree *)
+Admitted.
+
+Ltac crush_NoTemp :=
+  repeat match goal with
+    | [ H : Some (_, _) = DIRTREE.find_name [temp_fn] _ |- _ ] => 
+      rewrite find_name_delete_from_dir in H; congruence
+  end.
+
+Lemma NoTempFile_recover_ok : forall fsxp mscs,
+  {< m Fm Ftop src_tree src_dents tree dst_fn src_fn,
+   PRE
+     LOG.rep (FSXPLog fsxp) (sb_rep fsxp) (NoTransaction m) mscs *
+     [[ (Fm * DIRTREE.rep fsxp Ftop tree)%pred (list2mem m) ]] *
+     [[rep_tree NoTempFile src_tree src_dents tree src_fn dst_fn temp_fn]]
+   POST RET:mscs
+     atomic_cp_recover_rep fsxp Fm Ftop src_tree src_dents src_fn dst_fn mscs
+  CRASH
+    crash_transitions Fm Ftop fsxp src_tree src_dents src_fn dst_fn
+    >} atomic_cp_cleanup fsxp mscs.
+Proof.
+  unfold atomic_cp_cleanup, atomic_cp_recover_rep, rep_tree, rep_src_tree, rep_root; intros.
+  step.
+  step.
+  crush_NoTemp.
+  crush_NoTemp.
+  crush_NoTemp.
+  rewrite graft_root_is_add_root_dents.
+  rewrite delete_from_dir_add_dents; eauto.
+  (* maybe lemma for NoTemp2Temp *)
   unfold crash_transitions.
-  eapply pimpl_or_r. left.
+  apply pimpl_or_r; left.
   unfold rep_crash.
-  repeat (eapply pimpl_exists_r; eexists).
-  instantiate (x := m).
-  instantiate (x2 := tree).
   cancel.
-  eapply would_recover_either_pimpl_pred.
-  exists tree.
-  pred_apply.
-  cancel.
-  exists tree_elem.
-  intuition.
-  exists tree_elem.
+  rewrite graft_root_is_add_root_dents.
+  rewrite delete_from_dir_add_dents; eauto.
+  eapply UnChanged_ok.
+  unfold rep_src_tree, rep_tree, rep_root.
   intuition.
   Grab Existential Variables.
   all: eauto.
 Qed.
   
 Lemma TempFileExists_recover_ok : forall fsxp mscs,
-  {< m Fm Ftop tree dst_fn src_fn,
+  {< m Fm Ftop tree src_tree src_dents dst_fn src_fn,
    PRE
      LOG.rep (FSXPLog fsxp) (sb_rep fsxp) (NoTransaction m) mscs *
      [[ (Fm * DIRTREE.rep fsxp Ftop tree)%pred (list2mem m) ]] *
-     [[rep_tree TempFileExists tree src_fn dst_fn temp_fn]]
+     [[rep_tree TempFileExists src_tree src_dents tree src_fn dst_fn temp_fn]]
    POST RET:mscs
-     atomic_cp_recover_rep fsxp Fm Ftop src_fn dst_fn mscs
+     atomic_cp_recover_rep fsxp Fm Ftop src_tree src_dents src_fn dst_fn mscs
   CRASH
-    crash_transitions Fm Ftop fsxp src_fn dst_fn
+    crash_transitions Fm Ftop fsxp src_tree src_dents src_fn dst_fn
     >} atomic_cp_cleanup fsxp mscs.
 Proof.
-  unfold atomic_cp_cleanup. intros.
-  step.
-  eapply root_ok; eauto.
-  eapply root_ok; eauto.
+  unfold atomic_cp_cleanup, atomic_cp_recover_rep, rep_tree, rep_src_tree, rep_root; intros.
   step.
   step.
+  instantiate (pathname := []).
+  rewrite find_root_graft_dents; eauto.
   step.
-  step.
-  (* delete failed; FS bug spec; delete shouldn't fail *)
+  (* delete failed *)
   admit.
-  (* delete succeeded *)
-  unfold atomic_cp_recover_rep.
-  repeat (eapply pimpl_exists_r; eexists).
-  
-  instantiate (x := a4).
-  instantiate (x0 := tree).
-  instantiate (x1 := tree_elem).
-  instantiate (x2 := (DIRTREE.TreeDir the_dnum
-              (DIRTREE.delete_from_list temp_fn tree_elem))).
-  cancel.
-  cancel.
-  eapply pimpl_or_r; left.
-  cancel.
-  eapply find_name_delete_from_list with (dnum := the_dnum) (fn := temp_fn). 
+  rewrite graft_root_is_add_root_dents.
+  rewrite delete_from_dir_add_dents; eauto.
+  eapply TempFileExists_impl_Temp2NoTemp; auto.
+  unfold rep_src_tree, rep_root; eauto.
+  instantiate (tree' := DIRTREE.tree_graft the_dnum src_dents [] temp_fn telem
+          (DIRTREE.TreeDir the_dnum src_dents)); eauto.
+  eapply TempFileExists_ok; eauto.
+  unfold rep_src_tree, rep_root; eauto.
+  (* telem *)
+  admit.
+  (* delete failed *)
+  admit.
+  eapply temp_impl_Temp2Temp; eauto.
+  unfold rep_src_tree, rep_root; eauto.
+  unfold TempTree_mem.
+  pred_apply.
+  unfold TempTree_rep.
+  (* telem *)
+  admit.
+  Unshelve.
+  all: eauto.
 Admitted.
 
-
 Lemma DstFileExists_recover_ok : forall fsxp mscs,
-  {< m Fm Ftop tree dst_fn src_fn,
+  {< m Fm Ftop src_tree src_dents tree dst_fn src_fn,
    PRE
      LOG.rep (FSXPLog fsxp) (sb_rep fsxp) (NoTransaction m) mscs *
      [[ (Fm * DIRTREE.rep fsxp Ftop tree)%pred (list2mem m) ]] *
-     [[rep_tree DstFileExists tree src_fn dst_fn temp_fn]]
+     [[rep_tree DstFileExists src_tree src_dents tree src_fn dst_fn temp_fn]]
    POST RET:mscs
-     atomic_cp_recover_rep fsxp Fm Ftop src_fn dst_fn mscs
+     atomic_cp_recover_rep fsxp Fm Ftop src_tree src_dents src_fn dst_fn mscs
   CRASH
-    crash_transitions Fm Ftop fsxp src_fn dst_fn
+    crash_transitions Fm Ftop fsxp src_tree src_dents src_fn dst_fn
     >} atomic_cp_cleanup fsxp mscs.
 Proof.
-  unfold atomic_cp_cleanup; intros.
+  unfold atomic_cp_cleanup, atomic_cp_recover_rep; intros.
   step.
+  unfold rep_tree in H4.
+  intuition.
+  repeat (deex).
+  eauto.
+  unfold rep_tree in H4.
+  intuition.
+  repeat (deex).
+  eauto.
   step.
-  unfold atomic_cp_recover_rep.
-  repeat (eapply pimpl_exists_r; eexists).
-  instantiate (x := m).
-  instantiate (x0 := old_tree).
-  instantiate (x1 := tree_elem).
-  instantiate (x2 := (DIRTREE.tree_graft the_dnum tree_elem [] dst_fn
-             (DIRTREE.TreeFile new_inum bytes attr) old_tree)).
-  cancel.
-  cancel.
-  unfold crash_transitions.
-  eapply pimpl_or_r. right.
-  eapply pimpl_or_r. right.
-  eapply pimpl_or_r. right.
-  eapply pimpl_or_r. right.
-  eapply pimpl_or_r. right.
-  unfold rep_crash.
-  repeat (eapply pimpl_exists_r; eexists).
-  instantiate (x := m).
-  instantiate (x0 := (DIRTREE.tree_graft the_dnum tree_elem [] dst_fn
-                                         (DIRTREE.TreeFile new_inum bytes attr) old_tree)).
-  cancel.
-  eapply would_recover_either_pimpl_pred.
-  eexists.
-  instantiate (x := (DIRTREE.tree_graft the_dnum tree_elem [] dst_fn
-                                        (DIRTREE.TreeFile new_inum bytes attr) old_tree)).
-  pred_apply.
-  cancel.
-  exists old_tree.
-  exists old_inum.
-  exists new_inum.
-  exists bytes.
-  exists attr.
-  exists tree_elem.
-  split; eauto.
-  exists old_tree.
-  exists old_inum.
-  exists new_inum.
-  exists bytes.
-  exists attr.
-  exists tree_elem.
-  split; eauto.
-Qed.
+  unfold rep_tree in H4.
+  intuition.
+  repeat (deex).
+  instantiate (pathname := []).
+  admit.
+  step.
+  admit.
+  (* eapply Dst2Dst *)
+  admit.
+  admit.
+  (* DIRTREE.dirtree *)
+Admitted.
 
-
-(* Hint Extern 1 ({{_}} progseq (NoTempFile_cp_recover) _) => apply atomic_cp_recover_ok : prog. *)
 
 (* lift log_would_recover_either_pred through crash_xform *)
 Ltac lift_log_would_recover_either_pred :=
   unfold stars; simpl; repeat (rewrite crash_xform_exists_comm; norm'l; unfold stars; simpl);
   repeat (rewrite crash_xform_sep_star_dist); repeat (rewrite crash_xform_lift_empty); cancel.
 
+Ltac pg := match goal with
+            | [ |- ?x ] => idtac "g"  x
+          end.
+
+Ltac equate x y :=
+  let dummy := constr:(eq_refl x : x = y) in idtac.
+
+Ltac crush_pre a src_tree src_dents src_fn dst_fn:= 
+  match goal with
+   | [ |- LOG.rep _ _ (NoTransaction ?m0) _ * ?F_ =p=> ?F * LOG.rep _ _ (NoTransaction ?m1) _] => 
+    idtac "yyy"; equate F F_; equate m1 m0; subst a; cancel
+   | [ H: sep_star ?Fm (DIRTREE.rep _ ?Ftop ?tree) _ |- sep_star ?F (DIRTREE.rep _ ?top ?t) (list2mem _) ] => 
+    idtac "fm"; equate F Fm; equate top Ftop; subst a; equate t tree; eauto
+   | [ |- rep_tree _ ?s ?d _ ?sfn ?dfn _ ] => idtac "rep"; equate s src_tree; 
+       equate d src_dents; equate sfn src_fn; equate dfn dst_fn; eauto
+   | [ |- corr2 _ _ ] => step
+   | [ |- _ * crash_transitions _ _ _ _ _ _ _  =p=> _ ] => cancel
+  end.
+
+Ltac split_transition case1 case2 a src_tree src_dents src_fn dst_fn := 
+  repeat (setoid_rewrite sep_star_or_distr);
+  repeat (setoid_rewrite sep_star_or_distr_l);
+  eapply pimpl_or_split; 
+  eapply pimpl_ok2; 
+  [eapply case1 | 
+   cancel; try crush_pre a src_tree src_dents src_fn dst_fn | 
+   eapply case2 | 
+   cancel; try crush_pre a src_tree src_dents src_fn dst_fn
+  ].
+
+
 (* XXX shorten proof using automation *)
 Theorem atomic_cp_recover_ok :
-  {< fsxp Fm Ftop dst_fn src_fn,
+  {< fsxp Fm Ftop src_tree src_dents dst_fn src_fn,
    PRE
-    crash_xform (crash_transitions Fm Ftop fsxp src_fn dst_fn)
+    crash_xform (crash_transitions Fm Ftop fsxp src_tree src_dents src_fn dst_fn)
   POST RET:^(mscs, fsxp')
   [[ fsxp' = fsxp ]] *
-     atomic_cp_recover_rep fsxp Fm Ftop src_fn dst_fn mscs
+     atomic_cp_recover_rep fsxp Fm Ftop src_tree src_dents src_fn dst_fn mscs
   CRASH
-    crash_transitions Fm Ftop fsxp src_fn dst_fn
+    crash_transitions Fm Ftop fsxp src_tree src_dents src_fn dst_fn
     >} atomic_cp_recover.
 Proof.
-
   (* Pull the several crash transitions through crash_form so that we can deal
   with each case separately *)
 
@@ -1385,320 +1880,103 @@ Proof.
 
   (* step through recover but don't cancel immediately so that we arrange things
    so that we can prove each crash transition individually. *)
-
   eapply pimpl_ok2. eauto with prog.
-  unfold rep_crash.
-
   (* split all crash transition *)
   intros. norm'l. split_or_l.
 
-  (* first crash transition: NoTemp2NoTemp *)
+
+  (* first crash transition: Unchanged2Unchanged *)
   lift_log_would_recover_either_pred.
-  repeat (setoid_rewrite sep_star_or_distr).
-  repeat (setoid_rewrite sep_star_or_distr_l).
-  eapply pimpl_or_split.
-  eapply pimpl_ok2.
-  eapply NoTempFile_recover_ok.
-  cancel.
 
-  (*
-  Ltac Logrep fsxp x :=
-  match goal with
-    | [ H : ?a = fsxp |- LOG.rep (FSXPLog fsxp) (sb_rep fsxp) (NoTransaction x) ^( _, _) * _ =p=> _ * LOG.rep (FSXPLog ?a) (sb_rep ?a) (NoTransaction ?m) ^( _, _) ] => idtac "x"; rewrite H; instantiate (m := x)
-  end.
-
-  Logrep fsxp x.
-*)
-
-  instantiate (m:= x).
+  (* the first case is special .. *)
   instantiate (F_0 := F_).
-  instantiate (Ftop0 := Ftop).
-  rewrite H7.
-  cancel.
-  instantiate (tree := x0).
-  instantiate (Fm0 := Fm).
-  rewrite H7.
-  eauto.
-  exists tree_elem.
-  eauto.
-  step.
-  cancel.
+  instantiate (old := x).
+  instantiate (newpred := (Fm * DIRTREE.rep fsxp Ftop src_tree)%pred).
 
-  eapply pimpl_ok2.
-  eapply NoTempFile_recover_ok.
-  cancel.
-  exists tree_elem0.
-  intuition.
-  step.
-  cancel.
+  cancel; eapply crash_xform_pimpl; eapply would_recover_either_pimpl_pred; pred_apply; cancel.
+
+  split_transition UnChanged_recover_ok UnChanged_recover_ok a src_tree src_dents src_fn dst_fn.
   cancel.
   eapply pimpl_or_r; left.
-  cancel.
-  exists tree_elem; eauto.
+  admit.
 
-  (* NoTemp2Temp *)
+  (* second case: Unchanged2Temp *)
   lift_log_would_recover_either_pred.
-  repeat (setoid_rewrite sep_star_or_distr).
-  repeat (setoid_rewrite sep_star_or_distr_l).
-  eapply pimpl_or_split.
-  eapply pimpl_ok2.
-  eapply NoTempFile_recover_ok.
+  split_transition UnChanged_recover_ok TempFileExists_recover_ok a src_tree src_dents src_fn dst_fn.
   cancel.
-  instantiate (m:= x).
-  instantiate (F_0 := F_).
-  instantiate (Ftop0 := Ftop).
-  rewrite H7.
-  cancel.
-  instantiate (tree := x0).
-  instantiate (Fm0 := Fm).
-  rewrite H7.
-  eauto.
-  exists tree_elem.
-  eauto.
-  step.
-  cancel.
-
-  eapply pimpl_ok2.
-  eapply TempFileExists_recover_ok.
-  cancel.
-  exists tinum.
-  exists old_inum.
-  exists bytes.
-  exists attr.
-  exists tree_elem0.
-  instantiate (src_fn0 := src_fn).
-  intuition.
-  step.
+  apply pimpl_or_r; right.
+  apply pimpl_or_r; left.
+  exists x.
+  pred_apply.
   cancel.
   
-  cancel.
-  eapply pimpl_or_r; right.
-  eapply pimpl_or_r; left.
-  cancel.
-  exists tree_elem.
-  intuition.
-
-  (* next crash transition: Temp2NoTemp *)
+  (* third case: Temp2NoTemp *)
   lift_log_would_recover_either_pred.
-  repeat (setoid_rewrite sep_star_or_distr).
-  repeat (setoid_rewrite sep_star_or_distr_l).
-  eapply pimpl_or_split.
-  eapply pimpl_ok2.
-  eapply TempFileExists_recover_ok.
+  split_transition TempFileExists_recover_ok NoTempFile_recover_ok a src_tree src_dents src_fn dst_fn.
   cancel.
-  instantiate (m:= x).
-  instantiate (F_0 := F_).
-  cancel.
-  instantiate (Fm0 := Fm).
-  rewrite H8.
-  eauto.
-  exists tinum.
-  exists old_inum.
-  exists bytes.
-  exists attr.
-  exists tree_elem.
-  instantiate (src_fn0 := src_fn).
-  intuition.
-  step.
+  apply pimpl_or_r; right.
+  apply pimpl_or_r; right.
+  apply pimpl_or_r; left.
+  exists x.
+  pred_apply.
   cancel.
 
-  eapply pimpl_ok2.
-  eapply NoTempFile_recover_ok.
-  cancel.
-  exists tree_elem0.
-  intuition.
-  step.
-  cancel.
-  
-  cancel.
-  eapply pimpl_or_r; right.
-  eapply pimpl_or_r; right;
-  eapply pimpl_or_r; left.
-  cancel.
-  exists tinum.
-  exists old_inum.
-  exists bytes.
-  exists attr.
-  exists tree_elem.
-  eauto.
-         
+  (* 4th case: Temp2Temp *)
 
-  (* next crash transition: Temp2Temp *)
   lift_log_would_recover_either_pred.
-  repeat (setoid_rewrite sep_star_or_distr).
-  repeat (setoid_rewrite sep_star_or_distr_l).
-  eapply pimpl_or_split.
-  eapply pimpl_ok2.
-  eapply TempFileExists_recover_ok.
+  split_transition TempFileExists_recover_ok TempFileExists_recover_ok a src_tree src_dents src_fn dst_fn.
   cancel.
-  instantiate (m:= x).
-  instantiate (F_0 := F_).
-  cancel.
-  instantiate (Fm0 := Fm).
-  rewrite H8.
-  eauto.
-  exists tinum.
-  exists old_inum.
-  exists bytes.
-  exists attr.
-  exists tree_elem.
-  instantiate (src_fn0 := src_fn).
-  intuition.
-  step.
+  apply pimpl_or_r; right.
+  apply pimpl_or_r; right.
+  apply pimpl_or_r; right.
+  apply pimpl_or_r; left.
+  exists x.
+  pred_apply.
   cancel.
 
-  eapply pimpl_ok2.
-  eapply TempFileExists_recover_ok.
-  cancel.
-  exists tinum0.
-  exists old_inum0.
-  exists bytes0.
-  exists attr0.
-  exists tree_elem0.
-  instantiate (src_fn0 := src_fn).
-  intuition.
-  step.
-  cancel.
-
-  cancel.
-  eapply pimpl_or_r; right.
-  eapply pimpl_or_r; right;
-  eapply pimpl_or_r; right;
-  eapply pimpl_or_r; left.
-  cancel.
-  exists tinum.
-  exists old_inum.
-  exists bytes.
-  exists attr.
-  exists tree_elem.
-  eauto.
-
-  (* next transition: Temp2Dst *)
+  (* 5th case: Temp2Dst *) 
   lift_log_would_recover_either_pred.
-  repeat (setoid_rewrite sep_star_or_distr).
-  repeat (setoid_rewrite sep_star_or_distr_l).
-  eapply pimpl_or_split.
-  eapply pimpl_ok2.
-  eapply TempFileExists_recover_ok.
+  split_transition TempFileExists_recover_ok DstFileExists_recover_ok a src_tree src_dents src_fn dst_fn.
   cancel.
-  instantiate (m:= x).
-  instantiate (F_0 := F_).
+  apply pimpl_or_r; right.
+  apply pimpl_or_r; right.
+  apply pimpl_or_r; right.
+  apply pimpl_or_r; right.
+  apply pimpl_or_r; left.
+  exists x.
+  pred_apply.
   cancel.
-  instantiate (Fm0 := Fm).
-  instantiate (Ftop0 := Ftop).
-  instantiate (tree := x0).
-  rewrite H8; eauto.
-  exists tinum.
-  exists old_inum.
-  exists bytes.
-  exists attr.
-  exists tree_elem.
-  instantiate (src_fn0 := src_fn).
-  intuition.
-  step.
-  cancel.
-  
-  eapply pimpl_ok2.
-  eapply DstFileExists_recover_ok.
-  cancel.
-  exists old_tree.
-  exists old_inum0.
-  exists new_inum.
-  exists bytes0.
-  exists attr0.
-  exists tree_elem0.
-  instantiate (src_fn0 := src_fn).
-  intuition.
-  step.
-  cancel.
-
-  cancel.
-  eapply pimpl_or_r; right.
-  eapply pimpl_or_r; right;
-  eapply pimpl_or_r; right;
-  eapply pimpl_or_r; right;
-  eapply pimpl_or_r; left.
-  cancel.
-  exists tinum.
-  exists old_inum.
-  exists bytes.
-  exists attr.
-  exists tree_elem.
-  eauto.
 
   (* final transition Dst2Dst *)
-  
   lift_log_would_recover_either_pred.
-  repeat (setoid_rewrite sep_star_or_distr).
-  repeat (setoid_rewrite sep_star_or_distr_l).
-  eapply pimpl_or_split.
-  eapply pimpl_ok2.
-  eapply DstFileExists_recover_ok.
+  split_transition DstFileExists_recover_ok DstFileExists_recover_ok a src_tree src_dents src_fn dst_fn.
   cancel.
-  instantiate (m:= x).
-  instantiate (F_0 := F_).
+  apply pimpl_or_r; right.
+  apply pimpl_or_r; right.
+  apply pimpl_or_r; right.
+  apply pimpl_or_r; right.
+  apply pimpl_or_r; right.
+  exists x.
+  pred_apply.
   cancel.
-  instantiate (Fm0 := Fm).
-  instantiate (Ftop0 := Ftop).
-  instantiate (tree := (DIRTREE.tree_graft the_dnum tree_elem [] dst_fn
-            (DIRTREE.TreeFile new_inum bytes attr) old_tree)).
-  rewrite H9; eauto.
-  exists old_tree.
-  exists old_inum.
-  exists new_inum.
-  exists bytes.
-  exists attr.
-  exists tree_elem.
-  instantiate (src_fn0 := src_fn).
-  intuition.
-  step.
-  cancel.
-  
-  eapply pimpl_ok2.
-  eapply DstFileExists_recover_ok.
-  cancel.
-  exists old_tree0.
-  exists old_inum0.
-  exists new_inum0.
-  exists bytes0.
-  exists attr0.
-  exists tree_elem0.
-  instantiate (src_fn0 := src_fn).
-  intuition.
-  step.
-  cancel.
-
-  cancel.
-  eapply pimpl_or_r; right.
-  eapply pimpl_or_r; right.
-  eapply pimpl_or_r; right.
-  eapply pimpl_or_r; right.
-  eapply pimpl_or_r; right.
-  cancel.
-  exists old_tree.
-  exists old_inum.
-  exists new_inum.
-  exists bytes.
-  exists attr.
-  exists tree_elem.
-  eauto.
-Qed.
+Admitted.
 
 Hint Extern 1 ({{_}} progseq (atomic_cp_recover) _) => apply atomic_cp_recover_ok : prog.
 
 
 Theorem atomic_cp_with_recover_ok : forall fsxp src_fn dst_fn mscs,
-  {<< m Fm Ftop tree tree_elem,
+  {<< m Fm Ftop tree dents,
   PRE   LOG.rep (FSXPLog fsxp) (sb_rep fsxp) (NoTransaction m) mscs *
         [[ (Fm * DIRTREE.rep fsxp Ftop tree)%pred (list2mem m) ]] *
-        [[ tree = DIRTREE.TreeDir the_dnum tree_elem ]] *
+        [[ tree = DIRTREE.TreeDir the_dnum dents ]] *
         [[ DIRTREE.find_name [temp_fn] tree = None ]] *
         [[ src_fn <> temp_fn ]] *
-        [[ dst_fn <> temp_fn ]]
+        [[ dst_fn <> temp_fn ]] *
+        [[ src_fn <> dst_fn ]]
   POST RET:^(mscs, r)
-    atomic_cp_return_rep fsxp Fm Ftop tree tree_elem src_fn dst_fn mscs r
+    atomic_cp_return_rep fsxp Fm Ftop tree dents src_fn dst_fn mscs r
   REC RET:^(mscs,fsxp)
-    atomic_cp_recover_rep fsxp Fm Ftop src_fn dst_fn mscs
+    atomic_cp_recover_rep fsxp Fm Ftop src_tree src_dents src_fn dst_fn mscs
   >>} atomic_cp fsxp src_fn dst_fn mscs >> atomic_cp_recover.
 Proof.
   unfold forall_helper.
@@ -1708,10 +1986,13 @@ Proof.
   eauto with prog.
   eauto with prog.
   cancel.
+  unfold rep_src_tree, rep_root; intuition.
+  admit.
   eapply pimpl_ok2.
   eapply H2.
   cancel.
-  instantiate (crash :=(F_ *  crash_transitions v0 v1 fsxp src_fn dst_fn)%pred).
+  admit.
+  instantiate (crash :=(F_ *  crash_transitions v0 v1 fsxp v2 v3 src_fn dst_fn)%pred).
   subst; cancel.
   cancel.
   repeat (eapply pimpl_exists_r; eexists).
